Get Distributed/Common working with Dafny 3.0.0

ironfleet/src/Dafny/Distributed/Common/Framework/Environment.s.dfy
@@ -26,105 +26,105 @@ datatype LEnvironment<IdType, MessageType(==)> = LEnvironment(time:int,
                                         
 predicate IsValidLIoOp<IdType, MessageType>(io:LIoOp, actor:IdType, e:LEnvironment<IdType, MessageType>)
 {
-    match io
-        case LIoOpSend(s) => s.src == actor
-        case LIoOpReceive(r) => r.dst == actor
-        case LIoOpTimeoutReceive => true
-        case LIoOpReadClock(t) => true
+  match io
+    case LIoOpSend(s) => s.src == actor
+    case LIoOpReceive(r) => r.dst == actor
+    case LIoOpTimeoutReceive => true
+    case LIoOpReadClock(t) => true
 }
 
 predicate LIoOpOrderingOKForAction<IdType, MessageType>(
-    io1:LIoOp<IdType, MessageType>,
-    io2:LIoOp<IdType, MessageType>
-    )
+  io1:LIoOp<IdType, MessageType>,
+  io2:LIoOp<IdType, MessageType>
+  )
 {
-    io1.LIoOpReceive? || io2.LIoOpSend?
+  io1.LIoOpReceive? || io2.LIoOpSend?
 }
 
 predicate LIoOpSeqCompatibleWithReduction<IdType, MessageType>(
-    ios:seq<LIoOp<IdType, MessageType>>
-    )
+  ios:seq<LIoOp<IdType, MessageType>>
+  )
 {
-    forall i {:trigger ios[i], ios[i+1]} :: 0 <= i < |ios| - 1 ==> LIoOpOrderingOKForAction(ios[i], ios[i+1])
+  forall i {:trigger ios[i], ios[i+1]} :: 0 <= i < |ios| - 1 ==> LIoOpOrderingOKForAction(ios[i], ios[i+1])
 }
 
 predicate IsValidLEnvStep<IdType, MessageType>(e:LEnvironment<IdType, MessageType>, step:LEnvStep)
 {
-    match step
-        case LEnvStepHostIos(actor, ios) =>    (forall io :: io in ios ==> IsValidLIoOp(io, actor, e))
-                                           && LIoOpSeqCompatibleWithReduction(ios)
-        case LEnvStepDeliverPacket(p) => p in e.sentPackets
-        case LEnvStepAdvanceTime => true
-        case LEnvStepStutter => true
+  match step
+    case LEnvStepHostIos(actor, ios) => && (forall io :: io in ios ==> IsValidLIoOp(io, actor, e))
+                                        && LIoOpSeqCompatibleWithReduction(ios)
+    case LEnvStepDeliverPacket(p) => p in e.sentPackets
+    case LEnvStepAdvanceTime => true
+    case LEnvStepStutter => true
 }
 
 predicate LEnvironment_Init<IdType, MessageType>(
-    e:LEnvironment<IdType, MessageType>
-    )
+  e:LEnvironment<IdType, MessageType>
+  )
 {
-       |e.sentPackets| == 0
-    && e.time >= 0
+  && |e.sentPackets| == 0
+  && e.time >= 0
 }
 
 predicate LEnvironment_PerformIos<IdType, MessageType>(
-    e:LEnvironment<IdType, MessageType>,
-    e':LEnvironment<IdType, MessageType>,
-    actor:IdType,
-    ios:seq<LIoOp<IdType, MessageType>>
-    )
+  e:LEnvironment<IdType, MessageType>,
+  e':LEnvironment<IdType, MessageType>,
+  actor:IdType,
+  ios:seq<LIoOp<IdType, MessageType>>
+  )
 {
-       e'.sentPackets == e.sentPackets + (set io | io in ios && io.LIoOpSend? :: io.s)
-    && (forall io :: io in ios && io.LIoOpReceive? ==> io.r in e.sentPackets)
-    && e'.time == e.time
+  && e'.sentPackets == e.sentPackets + (set io | io in ios && io.LIoOpSend? :: io.s)
+  && (forall io :: io in ios && io.LIoOpReceive? ==> io.r in e.sentPackets)
+  && e'.time == e.time
 }
 
 predicate LEnvironment_AdvanceTime<IdType, MessageType>(
-    e:LEnvironment<IdType, MessageType>,
-    e':LEnvironment<IdType, MessageType>
-    )
+  e:LEnvironment<IdType, MessageType>,
+  e':LEnvironment<IdType, MessageType>
+  )
 {
-       e'.time > e.time
-    // UNCHANGED
-    && e'.sentPackets == e.sentPackets
+  && e'.time > e.time
+  // UNCHANGED
+  && e'.sentPackets == e.sentPackets
 }
 
 predicate LEnvironment_Stutter<IdType, MessageType>(
-    e:LEnvironment<IdType, MessageType>,
-    e':LEnvironment<IdType, MessageType>
-    )
+  e:LEnvironment<IdType, MessageType>,
+  e':LEnvironment<IdType, MessageType>
+  )
 {
-       e'.time == e.time
-    && e'.sentPackets == e.sentPackets
+  && e'.time == e.time
+  && e'.sentPackets == e.sentPackets
 }
 
 predicate LEnvironment_Next<IdType, MessageType>(
-    e:LEnvironment<IdType, MessageType>,
-    e':LEnvironment<IdType, MessageType>
-    )
+  e:LEnvironment<IdType, MessageType>,
+  e':LEnvironment<IdType, MessageType>
+  )
 {
-       IsValidLEnvStep(e, e.nextStep)
-    && match e.nextStep
-           case LEnvStepHostIos(actor, ios) => LEnvironment_PerformIos(e, e', actor, ios)
-           case LEnvStepDeliverPacket(p) => LEnvironment_Stutter(e, e') // this is only relevant for synchrony
-           case LEnvStepAdvanceTime => LEnvironment_AdvanceTime(e, e')
-           case LEnvStepStutter => LEnvironment_Stutter(e, e')
+  && IsValidLEnvStep(e, e.nextStep)
+  && match e.nextStep
+      case LEnvStepHostIos(actor, ios) => LEnvironment_PerformIos(e, e', actor, ios)
+      case LEnvStepDeliverPacket(p) => LEnvironment_Stutter(e, e') // this is only relevant for synchrony
+      case LEnvStepAdvanceTime => LEnvironment_AdvanceTime(e, e')
+      case LEnvStepStutter => LEnvironment_Stutter(e, e')
 }
 
 function{:opaque} EnvironmentNextTemporal<IdType,MessageType>(b:Behavior<LEnvironment<IdType, MessageType>>):temporal
-    requires imaptotal(b);
-    ensures forall i {:trigger sat(i, EnvironmentNextTemporal(b))} ::
-                sat(i, EnvironmentNextTemporal(b)) <==> LEnvironment_Next(b[i], b[i+1]);
+  requires imaptotal(b)
+  ensures forall i {:trigger sat(i, EnvironmentNextTemporal(b))} ::
+              sat(i, EnvironmentNextTemporal(b)) <==> LEnvironment_Next(b[i], b[i+1])
 {
-    stepmap(imap i :: LEnvironment_Next(b[i], b[i+1]))
+  stepmap(imap i :: LEnvironment_Next(b[i], b[i+1]))
 }
 
 predicate LEnvironment_BehaviorSatisfiesSpec<IdType, MessageType>(
-    b:Behavior<LEnvironment<IdType, MessageType>>
-    )
+  b:Behavior<LEnvironment<IdType, MessageType>>
+  )
 {
-       imaptotal(b)
-    && LEnvironment_Init(b[0])
-    && sat(0, always(EnvironmentNextTemporal(b)))
+  && imaptotal(b)
+  && LEnvironment_Init(b[0])
+  && sat(0, always(EnvironmentNextTemporal(b)))
 }
 
 } 
