ironfleet/src/Dafny/Distributed/Common/Framework/EnvironmentSynchronyLemmas.i.dfy
@@ -8,1151 +8,1178 @@ include "../../../Libraries/Math/mul_auto.i.dfy"
 include "../Collections/Sets.i.dfy"
 
 module Liveness__EnvironmentSynchronyLemmas_i {
+import opened Environment_s
 import opened EnvironmentSynchrony_s
 import opened Liveness__HostQueueLemmas_i
+import opened Temporal__Temporal_s
 import opened Temporal__Heuristics_i
+import opened Temporal__Monotonicity_i
 import opened Temporal__Rules_i
 import opened Temporal__Induction_i
+import opened Temporal__Time_s
 import opened Temporal__Time_i
 import opened Collections__Sets_i
+import opened Collections__Maps2_s
+import opened Collections__Maps2_i
 import opened Math__mul_auto_i
+import opened Math__mul_i
 
 function{:opaque} HostQueueEmptyTemporal<IdType, MessageType>(
-    b:Behavior<LEnvironment<IdType, MessageType>>,
-    host:IdType
-    ):temporal
-    requires imaptotal(b);
-    ensures  forall i {:trigger sat(i, HostQueueEmptyTemporal(b, host))} ::
-                 sat(i, HostQueueEmptyTemporal(b, host)) <==> (host in b[i].hostInfo ==> |b[i].hostInfo[host].queue| == 0);
+  b:Behavior<LEnvironment<IdType, MessageType>>,
+  host:IdType
+  ):temporal
+  requires imaptotal(b)
+  ensures  forall i {:trigger sat(i, HostQueueEmptyTemporal(b, host))} ::
+             sat(i, HostQueueEmptyTemporal(b, host)) <==> (host in b[i].hostInfo ==> |b[i].hostInfo[host].queue| == 0)
 {
-    stepmap(imap i :: host in b[i].hostInfo ==> |b[i].hostInfo[host].queue| == 0)
+  stepmap(imap i :: host in b[i].hostInfo ==> |b[i].hostInfo[host].queue| == 0)
 }
 
 function{:opaque} PacketInHostQueueTemporal<IdType, MessageType>(
-    b:Behavior<LEnvironment<IdType, MessageType>>,
-    p:LPacket<IdType, MessageType>
-    ):temporal
-    requires imaptotal(b);
-    ensures  forall i {:trigger sat(i, PacketInHostQueueTemporal(b, p))} :: sat(i, PacketInHostQueueTemporal(b, p)) <==>
-                                                                    (p.dst in b[i].hostInfo && p in b[i].hostInfo[p.dst].queue);
+  b:Behavior<LEnvironment<IdType, MessageType>>,
+  p:LPacket<IdType, MessageType>
+  ):temporal
+  requires imaptotal(b)
+  ensures  forall i {:trigger sat(i, PacketInHostQueueTemporal(b, p))} :: sat(i, PacketInHostQueueTemporal(b, p)) <==>
+                                                                  (p.dst in b[i].hostInfo && p in b[i].hostInfo[p.dst].queue)
 {
-    stepmap(imap i :: p.dst in b[i].hostInfo && p in b[i].hostInfo[p.dst].queue)
+  stepmap(imap i :: p.dst in b[i].hostInfo && p in b[i].hostInfo[p.dst].queue)
 }
 
 predicate PacketReceivedDuringAction<IdType, MessageType>(
-    e:LEnvironment<IdType, MessageType>,
-    p:LPacket<IdType, MessageType>
-    )
+  e:LEnvironment<IdType, MessageType>,
+  p:LPacket<IdType, MessageType>
+  )
 {
-    e.nextStep.LEnvStepHostIos? && LIoOpReceive(p) in e.nextStep.ios
+  e.nextStep.LEnvStepHostIos? && LIoOpReceive(p) in e.nextStep.ios
 }
 
 function{:opaque} PacketReceivedTemporal<IdType, MessageType>(
-    b:Behavior<LEnvironment<IdType, MessageType>>,
-    p:LPacket<IdType, MessageType>
-    ):temporal
-    requires imaptotal(b);
-    ensures  forall i {:trigger sat(i, PacketReceivedTemporal(b, p))} ::
-                 sat(i, PacketReceivedTemporal(b, p)) <==> PacketReceivedDuringAction(b[i], p);
+  b:Behavior<LEnvironment<IdType, MessageType>>,
+  p:LPacket<IdType, MessageType>
+  ):temporal
+  requires imaptotal(b)
+  ensures  forall i {:trigger sat(i, PacketReceivedTemporal(b, p))} ::
+             sat(i, PacketReceivedTemporal(b, p)) <==> PacketReceivedDuringAction(b[i], p)
 {
-    stepmap(imap i :: PacketReceivedDuringAction(b[i], p))
+  stepmap(imap i :: PacketReceivedDuringAction(b[i], p))
 }
 
-predicate AllPacketsReceivedWithin<IdType, MessageType>(
-    b:Behavior<LEnvironment<IdType, MessageType>>,
-    i:int,
-    receive_period:int,
-    sources:set<IdType>,
-    destinations:set<IdType>
-    )
-    requires imaptotal(b);
+predicate AllPacketsReceivedWithin<IdType(!new), MessageType(!new)>(
+  b:Behavior<LEnvironment<IdType, MessageType>>,
+  i:int,
+  receive_period:int,
+  sources:set<IdType>,
+  destinations:set<IdType>
+  )
+  requires imaptotal(b)
 {
-    forall p {:trigger PacketSentBetweenHosts(b[i], p, sources, destinations)} ::
-        PacketSentBetweenHosts(b[i], p, sources, destinations) ==>
-        sat(i, next(eventuallynextwithin(PacketReceivedTemporal(b, p), receive_period, BehaviorToTimeMap(b))))
+  forall p {:trigger PacketSentBetweenHosts(b[i], p, sources, destinations)} ::
+      PacketSentBetweenHosts(b[i], p, sources, destinations) ==>
+      sat(i, next(eventuallynextwithin(PacketReceivedTemporal(b, p), receive_period, BehaviorToTimeMap(b))))
 }
 
 function{:opaque} AllPacketsReceivedWithinTemporal<IdType, MessageType>(
-    b:Behavior<LEnvironment<IdType, MessageType>>,
-    receive_period:int,
-    sources:set<IdType>,
-    destinations:set<IdType>
-    ):temporal
-    requires imaptotal(b);
-    ensures  forall i {:trigger sat(i, AllPacketsReceivedWithinTemporal(b, receive_period, sources, destinations))} ::
-        sat(i, AllPacketsReceivedWithinTemporal(b, receive_period, sources, destinations)) <==>
-        AllPacketsReceivedWithin(b, i, receive_period, sources, destinations);
+  b:Behavior<LEnvironment<IdType, MessageType>>,
+  receive_period:int,
+  sources:set<IdType>,
+  destinations:set<IdType>
+  ):temporal
+  requires imaptotal(b)
+  ensures  forall i {:trigger sat(i, AllPacketsReceivedWithinTemporal(b, receive_period, sources, destinations))} ::
+             sat(i, AllPacketsReceivedWithinTemporal(b, receive_period, sources, destinations)) <==>
+             AllPacketsReceivedWithin(b, i, receive_period, sources, destinations)
 {
-    stepmap(imap i :: AllPacketsReceivedWithin(b, i, receive_period, sources, destinations))
+  stepmap(imap i :: AllPacketsReceivedWithin(b, i, receive_period, sources, destinations))
 }
 
 predicate ReceiveAttemptedInStep<IdType, MessageType>(
-    e:LEnvironment<IdType, MessageType>,
-    host:IdType
-    )
+  e:LEnvironment<IdType, MessageType>,
+  host:IdType
+  )
 {
-       e.nextStep.LEnvStepHostIos?
-    && e.nextStep.actor == host
-    && |e.nextStep.ios| > 0
-    && (e.nextStep.ios[0].LIoOpTimeoutReceive? || e.nextStep.ios[0].LIoOpReceive?)
+  && e.nextStep.LEnvStepHostIos?
+  && e.nextStep.actor == host
+  && |e.nextStep.ios| > 0
+  && (e.nextStep.ios[0].LIoOpTimeoutReceive? || e.nextStep.ios[0].LIoOpReceive?)
 }
 
 function{:opaque} ReceiveAttemptedTemporal<IdType, MessageType>(
-    b:Behavior<LEnvironment<IdType, MessageType>>,
-    host:IdType
-    ):temporal
-    requires imaptotal(b);
-    ensures  forall i {:trigger sat(i, ReceiveAttemptedTemporal(b, host))} ::
-                 sat(i, ReceiveAttemptedTemporal(b, host)) <==> ReceiveAttemptedInStep(b[i], host);
+  b:Behavior<LEnvironment<IdType, MessageType>>,
+  host:IdType
+  ):temporal
+  requires imaptotal(b)
+  ensures  forall i {:trigger sat(i, ReceiveAttemptedTemporal(b, host))} ::
+               sat(i, ReceiveAttemptedTemporal(b, host)) <==> ReceiveAttemptedInStep(b[i], host)
 {
-    stepmap(imap i :: ReceiveAttemptedInStep(b[i], host))
+  stepmap(imap i :: ReceiveAttemptedInStep(b[i], host))
 }
 
 lemma Lemma_TimeOnlyAdvancesBetweenSteps<IdType, MessageType>(
-    b:Behavior<LEnvironment<IdType, MessageType>>,
-    i:int,
-    j:int
-    )
-    requires LEnvironment_BehaviorSatisfiesSpec(b);
-    requires 0 <= i <= j;
-    ensures  b[i].time <= b[j].time;
-    decreases j - i;
+  b:Behavior<LEnvironment<IdType, MessageType>>,
+  i:int,
+  j:int
+  )
+  requires LEnvironment_BehaviorSatisfiesSpec(b)
+  requires 0 <= i <= j
+  ensures  b[i].time <= b[j].time
+  decreases j - i
 {
-    if j > i
-    {
-        Lemma_TimeOnlyAdvancesBetweenSteps(b, i, j-1);
-        TemporalDeduceFromAlways(0, j-1, EnvironmentNextTemporal(b));
-    }
+  if j > i
+  {
+    Lemma_TimeOnlyAdvancesBetweenSteps(b, i, j-1);
+    TemporalDeduceFromAlways(0, j-1, EnvironmentNextTemporal(b));
+  }
 }
 
 lemma Lemma_EstablishMonotonicFromOpaque<IdType, MessageType>(
-    b:Behavior<LEnvironment<IdType, MessageType>>,
-    start:int
-    )
-    requires LEnvironment_BehaviorSatisfiesSpec(b);
-    requires 0 <= start;
-    ensures  monotonic_from_opaque(start, BehaviorToTimeMap(b));
+  b:Behavior<LEnvironment<IdType, MessageType>>,
+  start:int
+  )
+  requires LEnvironment_BehaviorSatisfiesSpec(b)
+  requires 0 <= start
+  ensures  monotonic_from_opaque(start, BehaviorToTimeMap(b))
 {
-    var f := BehaviorToTimeMap(b);
-    forall i1, i2 | i1 in f && i2 in f && start <= i1 <= i2
-        ensures f[i1] <= f[i2];
-    {
-        Lemma_TimeOnlyAdvancesBetweenSteps(b, i1, i2);
-    }
-    reveal_monotonic_from_opaque();
+  var f := BehaviorToTimeMap(b);
+  forall i1, i2 | i1 in f && i2 in f && start <= i1 <= i2
+    ensures f[i1] <= f[i2]
+  {
+    Lemma_TimeOnlyAdvancesBetweenSteps(b, i1, i2);
+  }
+  reveal monotonic_from_opaque();
 }
 
 lemma Lemma_IfOpSeqIsCompatibleWithReductionAndFirstIsntReceiveThenNoneAreReceives2<IdType, MessageType>(
-    ios:seq<LIoOp<IdType, MessageType>>
-    )
-    requires LIoOpSeqCompatibleWithReduction(ios);
-    ensures  |ios| > 0 && !ios[0].LIoOpReceive? && !ios[0].LIoOpTimeoutReceive? ==> (forall io :: io in ios ==> !io.LIoOpReceive? && !io.LIoOpTimeoutReceive?);
+  ios:seq<LIoOp<IdType, MessageType>>
+  )
+  requires LIoOpSeqCompatibleWithReduction(ios)
+  ensures  |ios| > 0 && !ios[0].LIoOpReceive? && !ios[0].LIoOpTimeoutReceive? ==> (forall io :: io in ios ==> !io.LIoOpReceive? && !io.LIoOpTimeoutReceive?)
 {
-    if |ios| > 1 && !ios[0].LIoOpReceive? && !ios[0].LIoOpTimeoutReceive?
-    {
-        var i := 0;
-        assert 0 <= i < |ios| - 1;
-        assert LIoOpOrderingOKForAction(ios[i], ios[i+1]);
-        assert ios[1].LIoOpSend?;
-        Lemma_IfOpSeqIsCompatibleWithReductionThenSoIsSuffix(ios, 1);
-        Lemma_IfOpSeqIsCompatibleWithReductionAndFirstIsntReceiveThenNoneAreReceives2(ios[1..]);
-    }
+  if |ios| > 1 && !ios[0].LIoOpReceive? && !ios[0].LIoOpTimeoutReceive?
+  {
+    var i := 0;
+    assert 0 <= i < |ios| - 1;
+    assert LIoOpOrderingOKForAction(ios[i], ios[i+1]);
+    assert ios[1].LIoOpSend?;
+    Lemma_IfOpSeqIsCompatibleWithReductionThenSoIsSuffix(ios, 1);
+    Lemma_IfOpSeqIsCompatibleWithReductionAndFirstIsntReceiveThenNoneAreReceives2(ios[1..]);
+  }
 }
 
 lemma Lemma_ReceiveMakesHostQueueSmaller2<IdType, MessageType>(
-    q:seq<LPacket<IdType, MessageType>>,
-    q':seq<LPacket<IdType, MessageType>>,
-    ios:seq<LIoOp<IdType, MessageType>>,
-    io:LIoOp<IdType, MessageType>
-    )
-    requires HostQueue_PerformIos(q, q', ios);
-    requires LIoOpSeqCompatibleWithReduction(ios);
-    requires io.LIoOpTimeoutReceive? || io.LIoOpReceive?;
-    ensures  |q'| <= |q|;
-    ensures  io in ios ==> |q| == 0 || |q'| < |q|;
-    decreases |ios|;
+  q:seq<LPacket<IdType, MessageType>>,
+  q':seq<LPacket<IdType, MessageType>>,
+  ios:seq<LIoOp<IdType, MessageType>>,
+  io:LIoOp<IdType, MessageType>
+  )
+  requires HostQueue_PerformIos(q, q', ios)
+  requires LIoOpSeqCompatibleWithReduction(ios)
+  requires io.LIoOpTimeoutReceive? || io.LIoOpReceive?
+  ensures  |q'| <= |q|
+  ensures  io in ios ==> |q| == 0 || |q'| < |q|
+  decreases |ios|
 {
-    if (|ios| == 0)
-    {
-        assert q == q';
-        assert io !in ios;
-        return;
-    }
-    var io0 := ios[0];
-    assert ios == [io0] + ios[1..];
-    if (io0.LIoOpTimeoutReceive?)
-    {
-        assert |q| == 0;
-    }
-    else if (io0.LIoOpReceive?)
-    {
-        Lemma_IfOpSeqIsCompatibleWithReductionThenSoIsSuffix(ios, 1);
-        Lemma_ReceiveMakesHostQueueSmaller2(q[1..], q', ios[1..], io);
-    }
-    else
-    {
-        Lemma_IfOpSeqIsCompatibleWithReductionAndFirstIsntReceiveThenNoneAreReceives2(ios);
-    }
+  if (|ios| == 0)
+  {
+    assert q == q';
+    assert io !in ios;
+    return;
+  }
+  var io0 := ios[0];
+  assert ios == [io0] + ios[1..];
+  if (io0.LIoOpTimeoutReceive?)
+  {
+    assert |q| == 0;
+  }
+  else if (io0.LIoOpReceive?)
+  {
+    Lemma_IfOpSeqIsCompatibleWithReductionThenSoIsSuffix(ios, 1);
+    Lemma_ReceiveMakesHostQueueSmaller2(q[1..], q', ios[1..], io);
+  }
+  else
+  {
+    Lemma_IfOpSeqIsCompatibleWithReductionAndFirstIsntReceiveThenNoneAreReceives2(ios);
+  }
 }
 
 function{:opaque} QueuePosition<IdType, MessageType>(q:seq<LPacket<IdType, MessageType>>, p:LPacket<IdType, MessageType>):int
-    requires p in q;
-    ensures  0 <= QueuePosition(q, p) < |q|;
+  requires p in q
+  ensures  0 <= QueuePosition(q, p) < |q|
 {
-    if q[0] == p then 0
-    else 1 + QueuePosition(q[1..], p)
+  if q[0] == p then 0
+  else 1 + QueuePosition(q[1..], p)
 }
 
 lemma Lemma_QueuePosition<IdType, MessageType>(q:seq<LPacket<IdType, MessageType>>, p:LPacket<IdType, MessageType>)
-    requires p in q;
-    ensures QueuePosition(q, p) > 0 ==> |q| > 0 && p in q[1..] && QueuePosition(q[1..], p) < QueuePosition(q, p);
+  requires p in q
+  ensures QueuePosition(q, p) > 0 ==> |q| > 0 && p in q[1..] && QueuePosition(q[1..], p) < QueuePosition(q, p)
 {
-    reveal_QueuePosition();
+  reveal QueuePosition();
 }
 
-lemma Lemma_QueuePositionTail<IdType, MessageType>(q:seq<LPacket<IdType, MessageType>>, p:LPacket<IdType, MessageType>, q':seq<LPacket<IdType, MessageType>>)
-    requires p in q;
-    ensures  QueuePosition(q, p) == QueuePosition(q + q', p);
+lemma Lemma_QueuePositionTail<IdType, MessageType>(
+  q:seq<LPacket<IdType, MessageType>>,
+  p:LPacket<IdType, MessageType>,
+  q':seq<LPacket<IdType, MessageType>>
+  )
+  requires p in q
+  ensures  QueuePosition(q, p) == QueuePosition(q + q', p)
 {
-    reveal_QueuePosition();
-    if (q[0] == p)
-    {
-        assert QueuePosition(q, p) == QueuePosition(q + q', p);
-    }
-    else
-    {
-        Lemma_QueuePositionTail(q[1..], p, q');
-        assert q[1..] + q' == (q + q')[1..];
-    }
+  reveal QueuePosition();
+  if (q[0] == p)
+  {
+    assert QueuePosition(q, p) == QueuePosition(q + q', p);
+  }
+  else
+  {
+    Lemma_QueuePositionTail(q[1..], p, q');
+    assert q[1..] + q' == (q + q')[1..];
+  }
 }
 
 lemma Lemma_DeliverIsInstantaneous<IdType, MessageType>(
-    b:Behavior<LEnvironment<IdType, MessageType>>,
-    i:int,
-    host:IdType
-    )
-    requires LEnvironment_BehaviorSatisfiesSpec(b);
-    requires 0 <= i;
-    ensures  sat(i, always(ActionIsInstantaneousTemporal(PacketDeliveredToHostTemporal(b, host), BehaviorToTimeMap(b))));
+  b:Behavior<LEnvironment<IdType, MessageType>>,
+  i:int,
+  host:IdType
+  )
+  requires LEnvironment_BehaviorSatisfiesSpec(b)
+  requires 0 <= i
+  ensures  sat(i, always(ActionIsInstantaneousTemporal(PacketDeliveredToHostTemporal(b, host), BehaviorToTimeMap(b))))
 {
-    var x := PacketDeliveredToHostTemporal(b, host);
-    var f := BehaviorToTimeMap(b);
+  var x := PacketDeliveredToHostTemporal(b, host);
+  var f := BehaviorToTimeMap(b);
     
-    forall j | i <= j
-        ensures sat(j, ActionIsInstantaneousTemporal(x, f));
+  forall j | i <= j
+    ensures sat(j, ActionIsInstantaneousTemporal(x, f))
+  {
+    if sat(j, x)
     {
-        if sat(j, x)
-        {
-            TemporalDeduceFromAlways(0, j, EnvironmentNextTemporal(b));
-            assert f[j] == f[j+1];
-        }
+      TemporalDeduceFromAlways(0, j, EnvironmentNextTemporal(b));
+      assert f[j] == f[j+1];
     }
-    TemporalAlways(i, ActionIsInstantaneousTemporal(x, f));
+  }
+  TemporalAlways(i, ActionIsInstantaneousTemporal(x, f));
 }
 
 lemma Lemma_ReceiveIsInstantaneous<IdType, MessageType>(
-    b:Behavior<LEnvironment<IdType, MessageType>>,
-    i:int,
-    host:IdType
-    )
-    requires LEnvironment_BehaviorSatisfiesSpec(b);
-    requires 0 <= i;
-    ensures  sat(i, always(ActionIsInstantaneousTemporal(ReceiveAttemptedTemporal(b, host), BehaviorToTimeMap(b))));
+  b:Behavior<LEnvironment<IdType, MessageType>>,
+  i:int,
+  host:IdType
+  )
+  requires LEnvironment_BehaviorSatisfiesSpec(b)
+  requires 0 <= i
+  ensures  sat(i, always(ActionIsInstantaneousTemporal(ReceiveAttemptedTemporal(b, host), BehaviorToTimeMap(b))))
 {
-    var x := ReceiveAttemptedTemporal(b, host);
-    var f := BehaviorToTimeMap(b);
+  var x := ReceiveAttemptedTemporal(b, host);
+  var f := BehaviorToTimeMap(b);
     
-    forall j | i <= j
-        ensures sat(j, ActionIsInstantaneousTemporal(x, f));
+  forall j | i <= j
+    ensures sat(j, ActionIsInstantaneousTemporal(x, f));
+  {
+    if sat(j, x)
     {
-        if sat(j, x)
-        {
-            TemporalDeduceFromAlways(0, j, EnvironmentNextTemporal(b));
-            assert f[j] == f[j+1];
-        }
+      TemporalDeduceFromAlways(0, j, EnvironmentNextTemporal(b));
+      assert f[j] == f[j+1];
     }
-    TemporalAlways(i, ActionIsInstantaneousTemporal(x, f));
+  }
+  TemporalAlways(i, ActionIsInstantaneousTemporal(x, f));
 }
 
 
 lemma Lemma_DeliverIncrReceiveDecr<IdType, MessageType>(
-    i1:int,
-    i2:int,
-    b:Behavior<LEnvironment<IdType, MessageType>>,
-    host:IdType,
-    d:imap<int, int>
-    )
-    requires imaptotal(b);
-    requires imaptotal(d);
-    requires LEnvironment_BehaviorSatisfiesSpec(b);
-    requires HostQueuesLive(b);
-    requires TLe(0, i1);
-    requires TLe(i1, i2);
-    requires d[i1] >= 0;
-    requires d[i2] >= 1;
-    requires d == imap i :: if host in b[i].hostInfo then |b[i].hostInfo[host].queue| else 0;
-    ensures  (sat(i2, PacketDeliveredToHostTemporal(b, host)) && !sat(i2, ReceiveAttemptedTemporal(b, host)) && d[i2 + 1] == d[i2] + 1)
+  i1:int,
+  i2:int,
+  b:Behavior<LEnvironment<IdType, MessageType>>,
+  host:IdType,
+  d:imap<int, int>
+  )
+  requires imaptotal(b)
+  requires imaptotal(d)
+  requires LEnvironment_BehaviorSatisfiesSpec(b)
+  requires HostQueuesLive(b)
+  requires TLe(0, i1)
+  requires TLe(i1, i2)
+  requires d[i1] >= 0
+  requires d[i2] >= 1
+  requires d == imap i :: if host in b[i].hostInfo then |b[i].hostInfo[host].queue| else 0
+  ensures || (sat(i2, PacketDeliveredToHostTemporal(b, host)) && !sat(i2, ReceiveAttemptedTemporal(b, host)) && d[i2 + 1] == d[i2] + 1)
           || (!sat(i2, PacketDeliveredToHostTemporal(b, host)) && sat(i2, ReceiveAttemptedTemporal(b, host)) && d[i2 + 1] < d[i2])
-          || (!sat(i2, PacketDeliveredToHostTemporal(b, host)) && !sat(i2, ReceiveAttemptedTemporal(b, host)) && d[i2 + 1] == d[i2]);
+          || (!sat(i2, PacketDeliveredToHostTemporal(b, host)) && !sat(i2, ReceiveAttemptedTemporal(b, host)) && d[i2 + 1] == d[i2])
 {
-    TemporalAssist();
-    assert TLe(i1, i1);
-    var incr := PacketDeliveredToHostTemporal(b, host);
-    var decr := ReceiveAttemptedTemporal(b, host);
+  TemporalAssist();
+  assert TLe(i1, i1);
+  var incr := PacketDeliveredToHostTemporal(b, host);
+  var decr := ReceiveAttemptedTemporal(b, host);
 
-    assert TLe(0, i2);
-    assert i2 == i1 || TLe(i1, i2 - 1);
-    assert sat(i2, EnvironmentNextTemporal(b));
-    var e := b[i2];
-    var e' := b[i2 + 1];
-    assert LEnvironment_Next(e, e');
-    assert HostQueues_Next(e, e');
+  assert TLe(0, i2);
+  assert i2 == i1 || TLe(i1, i2 - 1);
+  assert sat(i2, EnvironmentNextTemporal(b));
+  var e := b[i2];
+  var e' := b[i2 + 1];
+  assert LEnvironment_Next(e, e');
+  assert HostQueues_Next(e, e');
 
-    assert 0 < d[i2];
-    assert host in e.hostInfo;
+  assert 0 < d[i2];
+  assert host in e.hostInfo;
 
-    var q := e.hostInfo[host].queue;
+  var q := e.hostInfo[host].queue;
 
-    if e.nextStep.LEnvStepHostIos?
+  if e.nextStep.LEnvStepHostIos?
+  {
+    if e.nextStep.actor != host
     {
-        if e.nextStep.actor != host
-        {
-            assert d[i2 + 1] == d[i2];
-        }
-        else if ReceiveAttemptedInStep(e, host)
-        {
-            var actor := e.nextStep.actor;
-            var ios := e.nextStep.ios;
-            var io := e.nextStep.ios[0];
-            var q' := e'.hostInfo[host].queue;
-            Lemma_ReceiveMakesHostQueueSmaller2(q, q', ios, io);
-            assert d[i2 + 1] < d[i2];
-        }
-        else
-        {
-            assert d[i2+1] == d[i2];
-        }
+      assert d[i2 + 1] == d[i2];
     }
-    else if e.nextStep.LEnvStepDeliverPacket?
+    else if ReceiveAttemptedInStep(e, host)
     {
-        var p := e.nextStep.p;
-        if (p.dst == host)
-        {
-            assert d[i2 + 1] == d[i2] + 1;
-        }
+      var actor := e.nextStep.actor;
+      var ios := e.nextStep.ios;
+      var io := e.nextStep.ios[0];
+      var q' := e'.hostInfo[host].queue;
+      Lemma_ReceiveMakesHostQueueSmaller2(q, q', ios, io);
+      assert d[i2 + 1] < d[i2];
     }
+    else
+    {
+      assert d[i2+1] == d[i2];
+    }
+  }
+  else if e.nextStep.LEnvStepDeliverPacket?
+  {
+    var p := e.nextStep.p;
+    if (p.dst == host)
+    {
+      assert d[i2 + 1] == d[i2] + 1;
+    }
+  }
 }
 
 // TODO: merge with Lemma_DeliverIncrReceiveDecr
 lemma Lemma_DeliverIncr<IdType, MessageType>(
-    i1:int,
-    i2:int,
-    b:Behavior<LEnvironment<IdType, MessageType>>,
-    host:IdType,
-    d:imap<int, int>
-    )
-    requires imaptotal(b);
-    requires imaptotal(d);
-    requires LEnvironment_BehaviorSatisfiesSpec(b);
-    requires HostQueuesLive(b);
-    requires TLe(0, i1);
-    requires TLe(i1, i2);
-    requires d[i1] >= 0;
-    requires d == imap i :: if host in b[i].hostInfo then |b[i].hostInfo[host].queue| else 0;
-    ensures  (sat(i2, PacketDeliveredToHostTemporal(b, host)) && d[i2 + 1] == d[i2] + 1)
-          || (!sat(i2, PacketDeliveredToHostTemporal(b, host)) && d[i2 + 1] <= d[i2]);
+  i1:int,
+  i2:int,
+  b:Behavior<LEnvironment<IdType, MessageType>>,
+  host:IdType,
+  d:imap<int, int>
+  )
+  requires imaptotal(b)
+  requires imaptotal(d)
+  requires LEnvironment_BehaviorSatisfiesSpec(b)
+  requires HostQueuesLive(b)
+  requires TLe(0, i1)
+  requires TLe(i1, i2)
+  requires d[i1] >= 0
+  requires d == imap i :: if host in b[i].hostInfo then |b[i].hostInfo[host].queue| else 0
+  ensures  || (sat(i2, PacketDeliveredToHostTemporal(b, host)) && d[i2 + 1] == d[i2] + 1)
+           || (!sat(i2, PacketDeliveredToHostTemporal(b, host)) && d[i2 + 1] <= d[i2])
 {
-    TemporalAssist();
-    assert TLe(i1, i1);
-    var incr := PacketDeliveredToHostTemporal(b, host);
-    var decr := ReceiveAttemptedTemporal(b, host);
+  TemporalAssist();
+  assert TLe(i1, i1);
+  var incr := PacketDeliveredToHostTemporal(b, host);
+  var decr := ReceiveAttemptedTemporal(b, host);
 
-    assert TLe(0, i2);
-    assert i2 == i1 || TLe(i1, i2 - 1);
-    assert sat(i2, EnvironmentNextTemporal(b));
-    var e := b[i2];
-    var e' := b[i2 + 1];
-    assert LEnvironment_Next(e, e');
-    assert HostQueues_Next(e, e');
+  assert TLe(0, i2);
+  assert i2 == i1 || TLe(i1, i2 - 1);
+  assert sat(i2, EnvironmentNextTemporal(b));
+  var e := b[i2];
+  var e' := b[i2 + 1];
+  assert LEnvironment_Next(e, e');
+  assert HostQueues_Next(e, e');
 
-    if (sat(i2, decr))
+  if (sat(i2, decr))
+  {
+    if (host in e.hostInfo)
     {
-        if (host in e.hostInfo)
+      var ios := e.nextStep.ios;
+      var io := e.nextStep.ios[0];
+      var q := e.hostInfo[host].queue;
+      var q' := e'.hostInfo[host].queue;
+      Lemma_ReceiveMakesHostQueueSmaller2(q, q', ios, io);
+      assert d[i2 + 1] <= d[i2];
+    }
+  }
+  else if e.nextStep.LEnvStepDeliverPacket?
+  {
+    var p := e.nextStep.p;
+    if (p.dst == host)
+    {
+      assert d[i2 + 1] == d[i2] + 1;
+    }
+  }
+  else if e.nextStep.LEnvStepAdvanceTime?
+  {
+    assert d[i2 + 1] == d[i2];
+  }
+  else if e.nextStep.LEnvStepHostIos?
+  {
+    assert !sat(i2, PacketDeliveredToHostTemporal(b, host));
+    var actor := e.nextStep.actor;
+    var ios := e.nextStep.ios;
+    if (host == actor)
+    {
+      if (!sat(i2+1, decr) && |ios| != 0)
+      {
+        if (ios[0].LIoOpReceive?)
         {
-            var ios := e.nextStep.ios;
-            var io := e.nextStep.ios[0];
-            var q := e.hostInfo[host].queue;
-            var q' := e'.hostInfo[host].queue;
-            Lemma_ReceiveMakesHostQueueSmaller2(q, q', ios, io);
-            assert d[i2 + 1] <= d[i2];
+          assert ReceiveAttemptedInStep(e, host);
         }
+      }
     }
-    else if e.nextStep.LEnvStepDeliverPacket?
-    {
-        var p := e.nextStep.p;
-        if (p.dst == host)
-        {
-            assert d[i2 + 1] == d[i2] + 1;
-        }
-    }
-    else if e.nextStep.LEnvStepAdvanceTime?
-    {
-        assert d[i2 + 1] == d[i2];
-    }
-    else if e.nextStep.LEnvStepHostIos?
-    {
-        assert !sat(i2, PacketDeliveredToHostTemporal(b, host));
-        var actor := e.nextStep.actor;
-        var ios := e.nextStep.ios;
-        if (host == actor)
-        {
-            if (!sat(i2+1, decr) && |ios| != 0)
-            {
-                if (ios[0].LIoOpReceive?)
-                {
-                    assert ReceiveAttemptedInStep(e, host);
-                }
-            }
-        }
-    }
+  }
 }
 
 lemma Lemma_HostQueueEmptiesAgain<IdType, MessageType>(
-    latency_bound:int,
-    host:IdType,
-    b:Behavior<LEnvironment<IdType, MessageType>>,
-    i1:int,
-    burst_size:int,
-    receive_period:int
-    ) returns(i2:int)
-    requires imaptotal(b);
-    requires LEnvironment_BehaviorSatisfiesSpec(b);
-    requires HostQueuesLive(b);
-    requires TLe(0, i1);
-    requires 1 <= receive_period;
-    requires 1 <= burst_size;
-    requires sat(i1, HostQueueEmptyTemporal(b, host));
-    requires sat(i1, always(eventuallynextwithin(ReceiveAttemptedTemporal(b, host), receive_period, BehaviorToTimeMap(b))));
-    requires sat(i1, always(NetworkDeliveryRateForHostBoundedTemporal(b, burst_size, burst_size * receive_period + 1, host)));
-    ensures  sat(i2, HostQueueEmptyTemporal(b, host));
-    ensures  i1 < i2;
-    ensures  forall i :: i1 <= i <= i2 && host in b[i].hostInfo ==> |b[i].hostInfo[host].queue| <= burst_size;
+  latency_bound:int,
+  host:IdType,
+  b:Behavior<LEnvironment<IdType, MessageType>>,
+  i1:int,
+  burst_size:int,
+  receive_period:int
+  ) returns(i2:int)
+  requires imaptotal(b)
+  requires LEnvironment_BehaviorSatisfiesSpec(b)
+  requires HostQueuesLive(b)
+  requires TLe(0, i1)
+  requires 1 <= receive_period
+  requires 1 <= burst_size
+  requires sat(i1, HostQueueEmptyTemporal(b, host))
+  requires sat(i1, always(eventuallynextwithin(ReceiveAttemptedTemporal(b, host), receive_period, BehaviorToTimeMap(b))))
+  requires sat(i1, always(NetworkDeliveryRateForHostBoundedTemporal(b, burst_size, burst_size * receive_period + 1, host)))
+  ensures  sat(i2, HostQueueEmptyTemporal(b, host))
+  ensures  i1 < i2
+  ensures  forall i :: i1 <= i <= i2 && host in b[i].hostInfo ==> |b[i].hostInfo[host].queue| <= burst_size
 {
-    var timefun := BehaviorToTimeMap(b);
-    var goal := HostQueueEmptyTemporal(b, host);
-    var d := imap i :: if host in b[i].hostInfo then |b[i].hostInfo[host].queue| else 0;
-    var bs := burst_size;
-    var r := receive_period;
-    var p := bs * r;
-    var incr := PacketDeliveredToHostTemporal(b, host);
-    var decr := ReceiveAttemptedTemporal(b, host);
-    var nIncr:int := bs;
-    var nDecr:int := bs;
-    TemporalAssist();
+  var timefun := BehaviorToTimeMap(b);
+  var goal := HostQueueEmptyTemporal(b, host);
+  var d := imap i :: if host in b[i].hostInfo then |b[i].hostInfo[host].queue| else 0;
+  var bs := burst_size;
+  var r := receive_period;
+  var p := bs * r;
+  var incr := PacketDeliveredToHostTemporal(b, host);
+  var decr := ReceiveAttemptedTemporal(b, host);
+  var nIncr:int := bs;
+  var nDecr:int := bs;
+  TemporalAssist();
 
-    Lemma_EstablishMonotonicFromOpaque(b, i1);
-    Lemma_DeliverIsInstantaneous(b, i1, host);
-    Lemma_ReceiveIsInstantaneous(b, i1, host);
+  Lemma_EstablishMonotonicFromOpaque(b, i1);
+  Lemma_DeliverIsInstantaneous(b, i1, host);
+  Lemma_ReceiveIsInstantaneous(b, i1, host);
 
-    forall ensures 1 <= p { lemma_mul_increases(bs, r); }
+  forall ensures 1 <= p { lemma_mul_increases(bs, r); }
 
+  assert TLe(i1, i1);
+  forall ensures sat(i1, countWithinGe(nDecr, decr, p, timefun))
+  {
+    Lemma_CountWithinGeOne(i1, decr, r, timefun);
+    Lemma_CountWithinGeMultiple(i1, bs, 1, decr, r, timefun);
+  }
+
+  forall ensures sat(i1, countWithinLe(nIncr, incr, p, timefun))
+  {
+    lemma_mul_is_commutative(bs, r);
+    assert sat(i1, always(NetworkDeliveryRateForHostBoundedTemporal(b, burst_size, burst_size * receive_period + 1, host)));
+    assert sat(i1, always(countWithinLe(bs, incr, p + 1, timefun)));
+    assert sat(i1, always(countWithinLe(bs, incr, p, timefun)));
+  }
+
+  if (d[i1 + 1] == 0)
+  {
+    i2 := i1 + 1;
+    return;
+  }
+
+  assert sat(i1, PacketDeliveredToHostTemporal(b, host));
+  assert sat(i1, ActionIsInstantaneousTemporal(PacketDeliveredToHostTemporal(b, host), timefun));
+  assert timefun[i1] == timefun[i1+1];
+  if (forall i :: TLe(i1, i) && i1 != i && timefun[i] <= timefun[i1] + p ==> d[i] > 0)
+  {
     assert TLe(i1, i1);
-    forall ensures sat(i1, countWithinGe(nDecr, decr, p, timefun));
+    forall i {:trigger TLe(i1, i)} | TLe(i1, i) && i1 != i && timefun[i] <= timefun[i1] + p
+      ensures || (sat(i, incr) && !sat(i, decr) && d[i + 1] == d[i] + 1)
+              || (!sat(i, incr) && sat(i, decr) && d[i + 1] < d[i])
+              || (!sat(i, incr) && !sat(i, decr) && d[i + 1] == d[i])
     {
-        Lemma_CountWithinGeOne(i1, decr, r, timefun);
-        Lemma_CountWithinGeMultiple(i1, bs, 1, decr, r, timefun);
+      Lemma_DeliverIncrReceiveDecr(i1, i, b, host, d);
     }
 
-    forall ensures sat(i1, countWithinLe(nIncr, incr, p, timefun));
+    forall ensures sat(i1, incr) && !sat(i1, decr) && d[i1 + 1] == d[i1] + 1
     {
-        lemma_mul_is_commutative(bs, r);
-        assert sat(i1, always(NetworkDeliveryRateForHostBoundedTemporal(b, burst_size, burst_size * receive_period + 1, host)));
-        assert sat(i1, always(countWithinLe(bs, incr, p + 1, timefun)));
-        assert sat(i1, always(countWithinLe(bs, incr, p, timefun)));
-    }
-
-    if (d[i1 + 1] == 0)
-    {
-        i2 := i1 + 1;
-        return;
-    }
-
-    assert sat(i1, PacketDeliveredToHostTemporal(b, host));
-    assert sat(i1, ActionIsInstantaneousTemporal(PacketDeliveredToHostTemporal(b, host), timefun));
-    assert timefun[i1] == timefun[i1+1];
-    if (forall i :: TLe(i1, i) && i1 != i && timefun[i] <= timefun[i1] + p ==> d[i] > 0)
-    {
-        assert TLe(i1, i1);
-        forall i {:trigger TLe(i1, i)} | TLe(i1, i) && i1 != i && timefun[i] <= timefun[i1] + p
-            ensures (sat(i, incr) && !sat(i, decr) && d[i + 1] == d[i] + 1)
-                 || (!sat(i, incr) && sat(i, decr) && d[i + 1] < d[i])
-                 || (!sat(i, incr) && !sat(i, decr) && d[i + 1] == d[i]);
+      if (!(host in b[i1].hostInfo))
+      {
+        assert !(host in b[i1 + 1].hostInfo);
+      }
+      if (sat(i1, decr))
+      {
+        if (host in b[i1].hostInfo)
         {
-            Lemma_DeliverIncrReceiveDecr(i1, i, b, host, d);
+          var ios := b[i1].nextStep.ios;
+          var io := ios[0];
+          Lemma_ReceiveMakesHostQueueSmaller2(b[i1].hostInfo[host].queue, b[i1 + 1].hostInfo[host].queue, ios, io);
         }
-
-        forall ensures sat(i1, incr) && !sat(i1, decr) && d[i1 + 1] == d[i1] + 1;
+        else
         {
-            if (!(host in b[i1].hostInfo))
-            {
-                assert !(host in b[i1 + 1].hostInfo);
-            }
-            if (sat(i1, decr))
-            {
-                if (host in b[i1].hostInfo)
-                {
-                    var ios := b[i1].nextStep.ios;
-                    var io := ios[0];
-                    Lemma_ReceiveMakesHostQueueSmaller2(b[i1].hostInfo[host].queue, b[i1 + 1].hostInfo[host].queue, ios, io);
-                }
-                else
-                {
-                }
-                assert false; // proof by contradiction
-            }
         }
-
-        i2 := Lemma_CountIncrDecr(i1, d, nIncr, nDecr, incr, decr, p, timefun);
-        var f1 := imap i :: d[i] <= d[i1] + nIncr - nDecr;
-        assert TLe(i1, i2) && sat(i2, stepmap(f1)) && timefun[i2] <= timefun[i1] + p;
-        assert d[i2] <= d[i1];
-        assert TLe(i1, i2);
-        assert i1 != i2;
-        assert timefun[i2] <= timefun[i1] + p;
-
         assert false; // proof by contradiction
+      }
     }
 
-    i2 :| i1 < i2 && timefun[i2] <= timefun[i1] + p && d[i2] == 0;
+    i2 := Lemma_CountIncrDecr(i1, d, nIncr, nDecr, incr, decr, p, timefun);
+    var f1 := imap i :: d[i] <= d[i1] + nIncr - nDecr;
+    assert TLe(i1, i2) && sat(i2, stepmap(f1)) && timefun[i2] <= timefun[i1] + p;
+    assert d[i2] <= d[i1];
+    assert TLe(i1, i2);
+    assert i1 != i2;
+    assert timefun[i2] <= timefun[i1] + p;
 
-    forall i {:trigger TLe(i1, i)} | TLe(i1, i) && timefun[i] <= timefun[i1] + p
-        ensures (sat(i, incr) && d[i + 1] == d[i] + 1)
-             || (!sat(i, incr) && d[i + 1] <= d[i]);
-    {
-        Lemma_DeliverIncr(i1, i, b, host, d);
-    }
-    Lemma_CountIncr(i1, d, nIncr, incr, p, timefun);
-    var f2 := imap i :: d[i] <= d[i1] + nIncr;
-    assert sat(i1, alwayswithin(stepmap(f2), p, timefun));
+    assert false; // proof by contradiction
+  }
 
-    forall i | i1 <= i <= i2 && host in b[i].hostInfo
-        ensures |b[i].hostInfo[host].queue| <= burst_size;
-    {
-        Lemma_TimeOnlyAdvancesBetweenSteps(b, i, i2);
-        TemporalDeduceFromAlways(i1, i, untilabsolutetime(stepmap(f2), timefun[i1] + p, timefun));
-        assert sat(i, stepmap(f2));
-    }
+  i2 :| i1 < i2 && timefun[i2] <= timefun[i1] + p && d[i2] == 0;
+
+  forall i {:trigger TLe(i1, i)} | TLe(i1, i) && timefun[i] <= timefun[i1] + p
+    ensures || (sat(i, incr) && d[i + 1] == d[i] + 1)
+            || (!sat(i, incr) && d[i + 1] <= d[i])
+  {
+    Lemma_DeliverIncr(i1, i, b, host, d);
+  }
+  Lemma_CountIncr(i1, d, nIncr, incr, p, timefun);
+  var f2 := imap i :: d[i] <= d[i1] + nIncr;
+  assert sat(i1, alwayswithin(stepmap(f2), p, timefun));
+
+  forall i | i1 <= i <= i2 && host in b[i].hostInfo
+    ensures |b[i].hostInfo[host].queue| <= burst_size
+  {
+    Lemma_TimeOnlyAdvancesBetweenSteps(b, i, i2);
+    TemporalDeduceFromAlways(i1, i, untilabsolutetime(stepmap(f2), timefun[i1] + p, timefun));
+    assert sat(i, stepmap(f2));
+  }
 }
 
 lemma Lemma_ReceiveAttemptNoDecr<IdType, MessageType>(
-    i2:int,
-    i3:int,
-    i4:int,
-    b:Behavior<LEnvironment<IdType, MessageType>>,
-    p:LPacket<IdType, MessageType>,
-    d:imap<int, int>,
-    r:int,
-    timefun:imap<int, int>
-    )   
-    requires imaptotal(b);
-    requires imaptotal(timefun);
-    requires LEnvironment_BehaviorSatisfiesSpec(b);
-    requires HostQueuesLive(b);
-    requires TLe(0, i2);
-    requires TLe(i2 + 1, i3);
-    ensures  TLe(i3, i4);
-    requires sat(i3, eventuallynextwithin(ReceiveAttemptedTemporal(b, p.dst), r, timefun));
-    requires d == imap i ::
+  i2:int,
+  i3:int,
+  i4:int,
+  b:Behavior<LEnvironment<IdType, MessageType>>,
+  p:LPacket<IdType, MessageType>,
+  d:imap<int, int>,
+  r:int,
+  timefun:imap<int, int>
+  )   
+  requires imaptotal(b)
+  requires imaptotal(timefun)
+  requires LEnvironment_BehaviorSatisfiesSpec(b)
+  requires HostQueuesLive(b)
+  requires TLe(0, i2)
+  requires TLe(i2 + 1, i3)
+  ensures  TLe(i3, i4)
+  requires sat(i3, eventuallynextwithin(ReceiveAttemptedTemporal(b, p.dst), r, timefun))
+  requires d == imap i ::
                 (if TLe(i2, i) && p.dst in b[i].hostInfo && p in b[i].hostInfo[p.dst].queue
                     then 1 + QueuePosition(b[i].hostInfo[p.dst].queue, p)
-                    else 0);
-    requires monotonic_from(i3, timefun);
-    requires i4 == earliestActionWithin(i3, ReceiveAttemptedTemporal(b, p.dst), r, timefun);
-    requires d[i3] >= 1;
-    ensures  d[i4] == d[i3];
-    decreases i4 - i3;
+                    else 0)
+  requires monotonic_from(i3, timefun)
+  requires i4 == earliestActionWithin(i3, ReceiveAttemptedTemporal(b, p.dst), r, timefun)
+  requires d[i3] >= 1
+  ensures  d[i4] == d[i3]
+  decreases i4 - i3
 {
-    TemporalAssist();
-    if (i3 < i4)
+  TemporalAssist();
+  if (i3 < i4)
+  {
+    assert TLe(0, i3);
+    var e := b[i3];
+    var e' := b[i3 + 1];
+    var q := e.hostInfo[p.dst].queue;
+    assert !sat(i3, ReceiveAttemptedTemporal(b, p.dst));
+
+    assert LEnvironment_Next(e, e');
+    assert HostQueues_Next(e, e');
+
+    if e.nextStep.LEnvStepDeliverPacket?
     {
-        assert TLe(0, i3);
-        var e := b[i3];
-        var e' := b[i3 + 1];
-        var q := e.hostInfo[p.dst].queue;
-        assert !sat(i3, ReceiveAttemptedTemporal(b, p.dst));
-
-        assert LEnvironment_Next(e, e');
-        assert HostQueues_Next(e, e');
-
-        if e.nextStep.LEnvStepDeliverPacket?
-        {
-            var q' := e'.hostInfo[p.dst].queue;
-            if (q != q')
-            {
-                var p' :| q' == q + [p'];
-                Lemma_QueuePositionTail(q, p, [p']);
-                assert d[i3] == d[i3 + 1];
-            }
-            assert d[i3] == d[i3 + 1];
-        }
-        else if e.nextStep.LEnvStepAdvanceTime?
-        {
-            assert d[i3] == d[i3 + 1];
-        }
-        else if e.nextStep.LEnvStepHostIos?
-        {
-            var actor := e.nextStep.actor;
-            var ios := e.nextStep.ios;
-            if (actor == p.dst)
-            {
-                var q' := e'.hostInfo[p.dst].queue;
-                assert HostQueue_PerformIos(q, q', ios);
-                if (|ios| > 0 && ios[0].LIoOpReceive?)
-                {
-                    var io := ios[0];
-                    assert ReceiveAttemptedInStep(e, p.dst);
-                }
-            }
-        }
-
+      var q' := e'.hostInfo[p.dst].queue;
+      if (q != q')
+      {
+        var p' :| q' == q + [p'];
+        Lemma_QueuePositionTail(q, p, [p']);
         assert d[i3] == d[i3 + 1];
-        Lemma_ReceiveAttemptNoDecr(i2, i3 + 1, i4, b, p, d, r, timefun);
+      }
+      assert d[i3] == d[i3 + 1];
     }
+    else if e.nextStep.LEnvStepAdvanceTime?
+    {
+      assert d[i3] == d[i3 + 1];
+    }
+    else if e.nextStep.LEnvStepHostIos?
+    {
+      var actor := e.nextStep.actor;
+      var ios := e.nextStep.ios;
+      if (actor == p.dst)
+      {
+        var q' := e'.hostInfo[p.dst].queue;
+        assert HostQueue_PerformIos(q, q', ios);
+        if (|ios| > 0 && ios[0].LIoOpReceive?)
+        {
+          var io := ios[0];
+          assert ReceiveAttemptedInStep(e, p.dst);
+        }
+      }
+    }
+
+    assert d[i3] == d[i3 + 1];
+    Lemma_ReceiveAttemptNoDecr(i2, i3 + 1, i4, b, p, d, r, timefun);
+  }
 }
 
 lemma Lemma_PromoteInQueue<IdType, MessageType>(
-    q:seq<LPacket<IdType, MessageType>>,
-    q':seq<LPacket<IdType, MessageType>>,
-    p:LPacket<IdType, MessageType>,
-    ios:seq<LIoOp<IdType, MessageType>>
-    )
-    requires p in q;
-    requires HostQueue_PerformIos(q, q', ios);
-    requires (forall i :: 0 <= i < |ios| && ios[i].LIoOpReceive? ==> ios[i].r != p);
-    ensures  p in q';
-    ensures  QueuePosition(q', p) <= QueuePosition(q, p);
-    ensures  |ios| >= 1 && ios[0].LIoOpReceive? ==> QueuePosition(q', p) < QueuePosition(q, p);
-    decreases ios;
+  q:seq<LPacket<IdType, MessageType>>,
+  q':seq<LPacket<IdType, MessageType>>,
+  p:LPacket<IdType, MessageType>,
+  ios:seq<LIoOp<IdType, MessageType>>
+  )
+  requires p in q
+  requires HostQueue_PerformIos(q, q', ios)
+  requires (forall i :: 0 <= i < |ios| && ios[i].LIoOpReceive? ==> ios[i].r != p)
+  ensures  p in q'
+  ensures  QueuePosition(q', p) <= QueuePosition(q, p)
+  ensures  |ios| >= 1 && ios[0].LIoOpReceive? ==> QueuePosition(q', p) < QueuePosition(q, p)
+  decreases ios
 {
-    reveal_QueuePosition();
-    if (|ios| > 0)
+  reveal QueuePosition();
+  if (|ios| > 0)
+  {
+    var io := ios[0];
+    if (io.LIoOpReceive?)
     {
-        var io := ios[0];
-        if (io.LIoOpReceive?)
-        {
-            Lemma_QueuePosition(q, p);
-            Lemma_PromoteInQueue(q[1..], q', p, ios[1..]);
-        }
+      Lemma_QueuePosition(q, p);
+      Lemma_PromoteInQueue(q[1..], q', p, ios[1..]);
     }
+  }
 }
 
 lemma Lemma_ReceiveAttemptDecr<IdType, MessageType>(
-    i2:int,
-    i3:int,
-    b:Behavior<LEnvironment<IdType, MessageType>>,
-    p:LPacket<IdType, MessageType>,
-    d:imap<int, int>,
-    r:int,
-    timefun:imap<int, int>
-    ) returns(i4:int)
-    requires imaptotal(b);
-    requires imaptotal(timefun);
-    requires LEnvironment_BehaviorSatisfiesSpec(b);
-    requires HostQueuesLive(b);
-    requires TLe(0, i2);
-    requires TLe(i2 + 1, i3);
-    requires monotonic_from(i3, timefun);
-    requires sat(i3, eventuallynextwithin(ReceiveAttemptedTemporal(b, p.dst), r, timefun));
-    requires d == imap i ::
+  i2:int,
+  i3:int,
+  b:Behavior<LEnvironment<IdType, MessageType>>,
+  p:LPacket<IdType, MessageType>,
+  d:imap<int, int>,
+  r:int,
+  timefun:imap<int, int>
+  ) returns(i4:int)
+  requires imaptotal(b)
+  requires imaptotal(timefun)
+  requires LEnvironment_BehaviorSatisfiesSpec(b)
+  requires HostQueuesLive(b)
+  requires TLe(0, i2)
+  requires TLe(i2 + 1, i3)
+  requires monotonic_from(i3, timefun)
+  requires sat(i3, eventuallynextwithin(ReceiveAttemptedTemporal(b, p.dst), r, timefun))
+  requires d == imap i ::
                 (if TLe(i2, i) && p.dst in b[i].hostInfo && p in b[i].hostInfo[p.dst].queue
                     then 1 + QueuePosition(b[i].hostInfo[p.dst].queue, p)
-                    else 0);
-    ensures  TLe(i3, i4);
-    ensures  sat(i3, actionGoalDecreaseWithin(PacketReceivedTemporal(b, p), d, r, timefun));
+                    else 0)
+  ensures  TLe(i3, i4)
+  ensures  sat(i3, actionGoalDecreaseWithin(PacketReceivedTemporal(b, p), d, r, timefun))
 {
-    TemporalAssist();
-    var goal := PacketReceivedTemporal(b, p);
+  TemporalAssist();
+  var goal := PacketReceivedTemporal(b, p);
 
-    i4 := earliestActionWithin(i3, ReceiveAttemptedTemporal(b, p.dst), r, timefun);
+  i4 := earliestActionWithin(i3, ReceiveAttemptedTemporal(b, p.dst), r, timefun);
 
-    if (d[i3] != 0)
-    {
-        assert d[i3] == (if TLe(i2, i3) && p.dst in b[i3].hostInfo && p in b[i3].hostInfo[p.dst].queue
+  if (d[i3] != 0)
+  {
+    assert d[i3] == (if TLe(i2, i3) && p.dst in b[i3].hostInfo && p in b[i3].hostInfo[p.dst].queue
                     then 1 + QueuePosition(b[i3].hostInfo[p.dst].queue, p)
                     else 0);
-        assert d[i3] > 0;
-        Lemma_ReceiveAttemptNoDecr(i2, i3, i4, b, p, d, r, timefun);
-        assert d[i3] == d[i4];
-        assert d[i4] > 0;
+    assert d[i3] > 0;
+    Lemma_ReceiveAttemptNoDecr(i2, i3, i4, b, p, d, r, timefun);
+    assert d[i3] == d[i4];
+    assert d[i4] > 0;
 
-        TemporalDeduceFromAlways(0, i4, HostQueuesNextTemporal(b));
-        var e := b[i4];
-        var e' := b[i4 + 1];
-        var ios := b[i4].nextStep.ios;
-        var io := ios[0];
-        var q := e.hostInfo[p.dst].queue;
-        Lemma_IfOpSeqIsCompatibleWithReductionAndFirstIsntReceiveThenNoneAreReceives2(ios);
-        assert io.LIoOpTimeoutReceive? || io.LIoOpReceive?;
+    TemporalDeduceFromAlways(0, i4, HostQueuesNextTemporal(b));
+    var e := b[i4];
+    var e' := b[i4 + 1];
+    var ios := b[i4].nextStep.ios;
+    var io := ios[0];
+    var q := e.hostInfo[p.dst].queue;
+    Lemma_IfOpSeqIsCompatibleWithReductionAndFirstIsntReceiveThenNoneAreReceives2(ios);
+    assert io.LIoOpTimeoutReceive? || io.LIoOpReceive?;
 
-        if (ios[0].LIoOpTimeoutReceive?)
-        {
-            assert |q| == 0;
-        }
-        if (ios[0].LIoOpReceive?)
-        {
-            assert p.dst in e'.hostInfo;
-            var q' := e'.hostInfo[p.dst].queue;
-            assert HostQueue_PerformIos(q, q', ios);
-            if (exists i :: 0 <= i < |ios| && ios[i].LIoOpReceive? && ios[i].r == p)
-            {
-                assert sat(i4, goal);
-            }
-            else
-            {
-                Lemma_PromoteInQueue(q, q', p, ios);
-                assert p in q' && QueuePosition(q', p) < QueuePosition(q, p);
-                assert (0 < d[i4 + 1] && d[i4 + 1] < d[i3]);
-            }
-        }
-
-        assert (0 < d[i4 + 1] && d[i4 + 1] < d[i3]) || sat(i4, goal);
-        assert sat(i3, actionGoalDecreaseWithin(PacketReceivedTemporal(b, p), d, r, timefun));
+    if (ios[0].LIoOpTimeoutReceive?)
+    {
+      assert |q| == 0;
+    }
+    if (ios[0].LIoOpReceive?)
+    {
+      assert p.dst in e'.hostInfo;
+      var q' := e'.hostInfo[p.dst].queue;
+      assert HostQueue_PerformIos(q, q', ios);
+      if (exists i :: 0 <= i < |ios| && ios[i].LIoOpReceive? && ios[i].r == p)
+      {
+        assert sat(i4, goal);
+      }
+      else
+      {
+        Lemma_PromoteInQueue(q, q', p, ios);
+        assert p in q' && QueuePosition(q', p) < QueuePosition(q, p);
+        assert (0 < d[i4 + 1] && d[i4 + 1] < d[i3]);
+      }
     }
 
+    assert (0 < d[i4 + 1] && d[i4 + 1] < d[i3]) || sat(i4, goal);
+    assert sat(i3, actionGoalDecreaseWithin(PacketReceivedTemporal(b, p), d, r, timefun));
+  }
 }
 
 lemma Lemma_HostQueueSizeBoundedAfterEmptyHelper<IdType, MessageType>(
-    latency_bound:int,
-    host:IdType,
-    b:Behavior<LEnvironment<IdType, MessageType>>,
-    i1:int,
-    i2:int,
-    burst_size:int,
-    receive_period:int
-    )
-    requires imaptotal(b);
-    requires LEnvironment_BehaviorSatisfiesSpec(b);
-    requires HostQueuesLive(b);
-    requires TLe(0, i1);
-    requires TLe(i1, i2);
-    requires 1 <= receive_period;
-    requires 1 <= burst_size;
-    requires sat(i1, HostQueueEmptyTemporal(b, host));
-    requires sat(i1, always(eventuallynextwithin(ReceiveAttemptedTemporal(b, host), receive_period, BehaviorToTimeMap(b))));
-    requires sat(i1, always(NetworkDeliveryRateForHostBoundedTemporal(b, burst_size, burst_size * receive_period + 1, host)));
-    ensures  forall i :: i1 <= i <= i2 && host in b[i].hostInfo ==> |b[i].hostInfo[host].queue| <= burst_size;
-    decreases i2 - i1;
+  latency_bound:int,
+  host:IdType,
+  b:Behavior<LEnvironment<IdType, MessageType>>,
+  i1:int,
+  i2:int,
+  burst_size:int,
+  receive_period:int
+  )
+  requires imaptotal(b)
+  requires LEnvironment_BehaviorSatisfiesSpec(b)
+  requires HostQueuesLive(b)
+  requires TLe(0, i1)
+  requires TLe(i1, i2)
+  requires 1 <= receive_period
+  requires 1 <= burst_size
+  requires sat(i1, HostQueueEmptyTemporal(b, host))
+  requires sat(i1, always(eventuallynextwithin(ReceiveAttemptedTemporal(b, host), receive_period, BehaviorToTimeMap(b))))
+  requires sat(i1, always(NetworkDeliveryRateForHostBoundedTemporal(b, burst_size, burst_size * receive_period + 1, host)))
+  ensures  forall i :: i1 <= i <= i2 && host in b[i].hostInfo ==> |b[i].hostInfo[host].queue| <= burst_size
+  decreases i2 - i1
 {
-    TemporalAssist();
-    Lemma_EstablishMonotonicFromOpaque(b, 0);
-    var i1' := Lemma_HostQueueEmptiesAgain(latency_bound, host, b, i1, burst_size, receive_period);
-    if (i1' < i2)
-    {
-        Lemma_HostQueueSizeBoundedAfterEmptyHelper(latency_bound, host, b, i1', i2, burst_size, receive_period);
-    }
+  TemporalAssist();
+  Lemma_EstablishMonotonicFromOpaque(b, 0);
+  var i1' := Lemma_HostQueueEmptiesAgain(latency_bound, host, b, i1, burst_size, receive_period);
+  if (i1' < i2)
+  {
+    Lemma_HostQueueSizeBoundedAfterEmptyHelper(latency_bound, host, b, i1', i2, burst_size, receive_period);
+  }
 }
 
 function{:opaque} QueueBounded<IdType, MessageType>(b:Behavior<LEnvironment<IdType, MessageType>>, host:IdType, burst_size:int):temporal
-    requires imaptotal(b);
-    ensures  forall i{:trigger sat(i, QueueBounded(b, host, burst_size))} ::
-        sat(i, QueueBounded(b, host, burst_size)) <==> (host in b[i].hostInfo ==> |b[i].hostInfo[host].queue| <= burst_size);
+  requires imaptotal(b)
+  ensures  forall i{:trigger sat(i, QueueBounded(b, host, burst_size))} ::
+             sat(i, QueueBounded(b, host, burst_size)) <==> (host in b[i].hostInfo ==> |b[i].hostInfo[host].queue| <= burst_size)
 {
-    stepmap(imap i :: host in b[i].hostInfo ==> |b[i].hostInfo[host].queue| <= burst_size)
+  stepmap(imap i :: host in b[i].hostInfo ==> |b[i].hostInfo[host].queue| <= burst_size)
 }
 
 lemma Lemma_HostQueueSizeBoundedAfterEmpty<IdType, MessageType>(
-    latency_bound:int,
-    host:IdType,
-    b:Behavior<LEnvironment<IdType, MessageType>>,
-    i1:int,
-    burst_size:int,
-    receive_period:int
-    )
-    requires imaptotal(b);
-    requires LEnvironment_BehaviorSatisfiesSpec(b);
-    requires HostQueuesLive(b);
-    requires TLe(0, i1);
-    requires 1 <= receive_period;
-    requires 1 <= burst_size;
-    requires sat(i1, HostQueueEmptyTemporal(b, host));
-    requires sat(i1, always(eventuallynextwithin(ReceiveAttemptedTemporal(b, host), receive_period, BehaviorToTimeMap(b))));
-    requires sat(i1, always(NetworkDeliveryRateForHostBoundedTemporal(b, burst_size, burst_size * receive_period + 1, host)));
-    ensures  sat(i1, always(QueueBounded(b, host, burst_size)));
+  latency_bound:int,
+  host:IdType,
+  b:Behavior<LEnvironment<IdType, MessageType>>,
+  i1:int,
+  burst_size:int,
+  receive_period:int
+  )
+  requires imaptotal(b)
+  requires LEnvironment_BehaviorSatisfiesSpec(b)
+  requires HostQueuesLive(b)
+  requires TLe(0, i1)
+  requires 1 <= receive_period
+  requires 1 <= burst_size
+  requires sat(i1, HostQueueEmptyTemporal(b, host))
+  requires sat(i1, always(eventuallynextwithin(ReceiveAttemptedTemporal(b, host), receive_period, BehaviorToTimeMap(b))))
+  requires sat(i1, always(NetworkDeliveryRateForHostBoundedTemporal(b, burst_size, burst_size * receive_period + 1, host)))
+  ensures  sat(i1, always(QueueBounded(b, host, burst_size)))
 {
-    TemporalAssist();
-    forall i2 | TLe(i1, i2)
-        ensures sat(i2, QueueBounded(b, host, burst_size))
+  TemporalAssist();
+  forall i2 | TLe(i1, i2)
+    ensures sat(i2, QueueBounded(b, host, burst_size))
+  {
+    if (host in b[i2].hostInfo)
     {
-        if (host in b[i2].hostInfo)
-        {
-            Lemma_HostQueueSizeBoundedAfterEmptyHelper(latency_bound, host, b, i1, i2, burst_size, receive_period);
-            assert |b[i2].hostInfo[host].queue| <= burst_size;
-        }
-        assert host in b[i2].hostInfo ==> |b[i2].hostInfo[host].queue| <= burst_size;
-        assert sat(i2, stepmap(imap i :: host in b[i].hostInfo ==> |b[i].hostInfo[host].queue| <= burst_size));
-        assert sat(i2, QueueBounded(b, host, burst_size));
+      Lemma_HostQueueSizeBoundedAfterEmptyHelper(latency_bound, host, b, i1, i2, burst_size, receive_period);
+      assert |b[i2].hostInfo[host].queue| <= burst_size;
     }
-    assert sat(i1, always(QueueBounded(b, host, burst_size)));
+    assert host in b[i2].hostInfo ==> |b[i2].hostInfo[host].queue| <= burst_size;
+    assert sat(i2, stepmap(imap i :: host in b[i].hostInfo ==> |b[i].hostInfo[host].queue| <= burst_size));
+    assert sat(i2, QueueBounded(b, host, burst_size));
+  }
+  assert sat(i1, always(QueueBounded(b, host, burst_size)));
 }
 
 lemma Lemma_EventuallyEachHostQueueEmpties<IdType, MessageType>(
-    latency_bound:int,
-    destinations:set<IdType>,
-    b:Behavior<LEnvironment<IdType, MessageType>>,
-    synchrony_start:int,
-    burst_size:int,
-    receive_period:int
-    )
-    requires imaptotal(b);
-    requires LEnvironment_BehaviorSatisfiesSpec(b);
-    requires HostQueuesLive(b);
-    requires TLe(0, synchrony_start);
-    requires 1 <= receive_period;
-    requires 1 <= burst_size;
+  latency_bound:int,
+  destinations:set<IdType>,
+  b:Behavior<LEnvironment<IdType, MessageType>>,
+  synchrony_start:int,
+  burst_size:int,
+  receive_period:int
+  )
+  requires imaptotal(b)
+  requires LEnvironment_BehaviorSatisfiesSpec(b)
+  requires HostQueuesLive(b)
+  requires TLe(0, synchrony_start)
+  requires 1 <= receive_period
+  requires 1 <= burst_size
 
-    // Starting from the synchrony point, each host attempts to receive a packet at least once every receive_period.
-    // That is, it performs an I/O that's either a Receive or a TimeoutReceive.
-    requires forall host :: host in destinations ==> sat(synchrony_start, always(eventuallynextwithin(ReceiveAttemptedTemporal(b, host), receive_period, BehaviorToTimeMap(b))));
+  // Starting from the synchrony point, each host attempts to receive a packet at least once every receive_period.
+  // That is, it performs an I/O that's either a Receive or a TimeoutReceive.
+  requires forall host :: host in destinations ==> sat(synchrony_start, always(eventuallynextwithin(ReceiveAttemptedTemporal(b, host), receive_period, BehaviorToTimeMap(b))))
 
-    // Starting from the synchrony point, the network stops overwhelming each host with
-    // delivered packets.  That is, there are at most burst_size packets delivered to any host during any period
-    // of length <= burst_size * receive_period + 1
-    requires forall host :: host in destinations ==> sat(synchrony_start, always(NetworkDeliveryRateForHostBoundedTemporal(b, burst_size, burst_size * receive_period + 1, host)));
+  // Starting from the synchrony point, the network stops overwhelming each host with
+  // delivered packets.  That is, there are at most burst_size packets delivered to any host during any period
+  // of length <= burst_size * receive_period + 1
+  requires forall host :: host in destinations ==> sat(synchrony_start, always(NetworkDeliveryRateForHostBoundedTemporal(b, burst_size, burst_size * receive_period + 1, host)))
 
-    // At some point after the synchrony point, possibly different for each host, that host's queue becomes empty.
-    ensures  forall host:: host in destinations ==> sat(synchrony_start, eventual(HostQueueEmptyTemporal(b, host)));
+  // At some point after the synchrony point, possibly different for each host, that host's queue becomes empty.
+  ensures  forall host:: host in destinations ==> sat(synchrony_start, eventual(HostQueueEmptyTemporal(b, host)))
 {
-    var timefun := BehaviorToTimeMap(b);
+  var timefun := BehaviorToTimeMap(b);
 
-    forall host | host in destinations
-        ensures sat(synchrony_start, eventual(HostQueueEmptyTemporal(b, host)));
+  forall host | host in destinations
+    ensures sat(synchrony_start, eventual(HostQueueEmptyTemporal(b, host)))
+  {
+    // If   []t :: <>(goal || d' < d[t]')
+    // and  [](0 <= d)
+    // then []<>(goal)
+    // goal = (|Q| == 0)
+    // d = |Q|
+    var i0 := synchrony_start;
+    var goal := HostQueueEmptyTemporal(b, host);
+
+    var d := imap i :: if host in b[i].hostInfo then |b[i].hostInfo[host].queue| else 0;
+
+    TemporalAssist();
+    var start := i0;
+    forall i1 | TLe(i0, i1)
+      ensures sat(i1, nextOrDecrease(goal, d))
     {
-        // If   []t :: <>(goal || d' < d[t]')
-        // and  [](0 <= d)
-        // then []<>(goal)
-        // goal = (|Q| == 0)
-        // d = |Q|
-        var i0 := synchrony_start;
-        var goal := HostQueueEmptyTemporal(b, host);
+      if (!sat(i1, eventual(or(goal, nextDecrease(i1, d)))))
+      {
+        assert forall i :: TLe(i1, i) ==> !sat(i, goal);
+        assert forall i :: TLe(i1, i) ==> !sat(i, nextDecrease(i1, d));
+        assert forall i :: TLe(i1, i) ==> d[i + 1] >= d[i1];
+        assert TLe(i1, i1);
+        assert !sat(i1, HostQueueEmptyTemporal(b, host));
+        assert !(host in b[i1].hostInfo ==> |b[i1].hostInfo[host].queue| == 0);
+        assert d[i1] > 0;
 
-        var d := imap i :: if host in b[i].hostInfo then |b[i].hostInfo[host].queue| else 0;
+        Lemma_EstablishMonotonicFromOpaque(b, i1);
 
-        TemporalAssist();
-        var start := i0;
-        forall i1 | TLe(i0, i1)
-            ensures sat(i1, nextOrDecrease(goal, d));
+        var bs := burst_size;
+        var r := receive_period;
+        var p := bs * r;
+        forall ensures 1 <= p { lemma_mul_increases(bs, r); }
+        forall ensures 0 <= p * (p + 1) { lemma_mul_nonnegative(p, p + 1); }
+        forall ensures p * (p + 1) == (p + 1) * p { lemma_mul_auto(); }
+        forall ensures bs * p < bs * (p + 1) { lemma_mul_auto(); }
+
+        // In time p * (p + 1), we'll deliver >= bs * (p + 1) messages
+        // In time (p + 1) * p, we'll receive <= bs * p messages
+        // So in time p * (p + 1) == (p + 1) * p, we'll decrease d by bs
+
+        // use d >= 1 to prove that delivery decrements
+        // define decr_action as d' = d - 1
+        // define incr_action as d' = d + 1
+        // p * (p + 1): |decr_action| >= bs * (p + 1)
+        //   p: |decr_action| >= bs
+        //     r: |decr_action| >= 1
+        // (p * 1) * p: |incr_action| <= bs * p
+        //   p + 1: |incr_action| <= bs
+        // d' = d + |incr_action| - |decr_action|
+        var incr := PacketDeliveredToHostTemporal(b, host);
+        var decr := ReceiveAttemptedTemporal(b, host);
+
+        assert TLe(i1, i1);
+        forall ensures sat(i1, countWithinGe(bs * (p + 1), decr, p * (p + 1), timefun))
         {
-            if (!sat(i1, eventual(or(goal, nextDecrease(i1, d)))))
-            {
-                assert forall i :: TLe(i1, i) ==> !sat(i, goal);
-                assert forall i :: TLe(i1, i) ==> !sat(i, nextDecrease(i1, d));
-                assert forall i :: TLe(i1, i) ==> d[i + 1] >= d[i1];
-                assert TLe(i1, i1);
-                assert !sat(i1, HostQueueEmptyTemporal(b, host));
-                assert !(host in b[i1].hostInfo ==> |b[i1].hostInfo[host].queue| == 0);
-                assert d[i1] > 0;
-
-                Lemma_EstablishMonotonicFromOpaque(b, i1);
-
-                var bs := burst_size;
-                var r := receive_period;
-                var p := bs * r;
-                forall ensures 1 <= p { lemma_mul_increases(bs, r); }
-                forall ensures 0 <= p * (p + 1) { lemma_mul_nonnegative(p, p + 1); }
-                forall ensures p * (p + 1) == (p + 1) * p { lemma_mul_auto(); }
-                forall ensures bs * p < bs * (p + 1) { lemma_mul_auto(); }
-
-                // In time p * (p + 1), we'll deliver >= bs * (p + 1) messages
-                // In time (p + 1) * p, we'll receive <= bs * p messages
-                // So in time p * (p + 1) == (p + 1) * p, we'll decrease d by bs
-
-                // use d >= 1 to prove that delivery decrements
-                // define decr_action as d' = d - 1
-                // define incr_action as d' = d + 1
-                // p * (p + 1): |decr_action| >= bs * (p + 1)
-                //   p: |decr_action| >= bs
-                //     r: |decr_action| >= 1
-                // (p * 1) * p: |incr_action| <= bs * p
-                //   p + 1: |incr_action| <= bs
-                // d' = d + |incr_action| - |decr_action|
-                var incr := PacketDeliveredToHostTemporal(b, host);
-                var decr := ReceiveAttemptedTemporal(b, host);
-
-                assert TLe(i1, i1);
-                forall ensures sat(i1, countWithinGe(bs * (p + 1), decr, p * (p + 1), timefun));
-                {
-                    Lemma_CountWithinGeOne(i1, decr, r, timefun);
-                    Lemma_CountWithinGeMultiple(i1, bs, 1, decr, r, timefun);
-                    Lemma_CountWithinGeMultiple(i1, p + 1, bs, decr, p, timefun);
-                }
-                
-                forall ensures sat(i1, countWithinLe(bs * p, incr, (p + 1) * p, timefun));
-                {
-                    assert sat(synchrony_start, always(NetworkDeliveryRateForHostBoundedTemporal(b, burst_size, burst_size * receive_period + 1, host)));
-                    assert sat(i1, always(NetworkDeliveryRateForHostBoundedTemporal(b, burst_size, burst_size * receive_period + 1, host)));
-                    assert sat(i1, always(countWithinLe(bs, incr, p + 1, timefun)));
-                    Lemma_DeliverIsInstantaneous(b, i1, host);
-                    Lemma_CountWithinLeMultiple(i1, p, bs, incr, p + 1, timefun);
-                }
-
-                var nIncr:int := bs * p;
-                var nDecr:int := bs * (p + 1);
-                var span := p * (p + 1);
-                assert sat(i1, countWithinLe(nIncr, incr, span, timefun));
-                assert sat(i1, countWithinGe(nDecr, decr, span, timefun));
-
-                forall i2 {:trigger TLe(i1, i2)} | TLe(i1, i2)
-                    ensures (sat(i2, PacketDeliveredToHostTemporal(b, host)) && !sat(i2, ReceiveAttemptedTemporal(b, host)) && d[i2 + 1] == d[i2] + 1)
-                         || (!sat(i2, PacketDeliveredToHostTemporal(b, host)) && sat(i2, ReceiveAttemptedTemporal(b, host)) && d[i2 + 1] < d[i2])
-                         || (!sat(i2, PacketDeliveredToHostTemporal(b, host)) && !sat(i2, ReceiveAttemptedTemporal(b, host)) && d[i2 + 1] == d[i2]);
-                {
-                    Lemma_DeliverIncrReceiveDecr(i1, i2, b, host, d);
-                }
-
-                var i2 := Lemma_CountIncrDecr(i1, d, nIncr, nDecr, incr, decr, span, timefun);
-                assert nDecr > 0;
-                assert TLe(i1, i2 - 1);
-                assert false; // proof by contradiction
-            }
-            var i2 :| TLe(i1, i2) && sat(i2, or(goal, nextDecrease(i1, d)));
-            assert sat(i1, eventual(or(goal, nextDecrease(i1, d))));
+          Lemma_CountWithinGeOne(i1, decr, r, timefun);
+          Lemma_CountWithinGeMultiple(i1, bs, 1, decr, r, timefun);
+          Lemma_CountWithinGeMultiple(i1, p + 1, bs, decr, p, timefun);
         }
-        assert imaptotal(d);
-        assert forall i :: start <= i ==> 0 <= d[i];
-        assert sat(start, always(nextOrDecrease(goal, d)));
-        Lemma_EventuallyNext(i0, d, goal);
-        assert sat(start, always(eventual(goal)));
+                
+        forall ensures sat(i1, countWithinLe(bs * p, incr, p * (p + 1), timefun))
+        {
+          assert sat(synchrony_start,
+                     always(NetworkDeliveryRateForHostBoundedTemporal(b, burst_size, burst_size * receive_period + 1, host)));
+          assert sat(i1, always(NetworkDeliveryRateForHostBoundedTemporal(b, burst_size, burst_size * receive_period + 1, host)));
+          assert sat(i1, always(countWithinLe(bs, incr, p + 1, timefun)));
+          Lemma_DeliverIsInstantaneous(b, i1, host);
+          Lemma_CountWithinLeMultiple(i1, p, bs, incr, p + 1, timefun);
+        }
+
+        var nIncr:int := bs * p;
+        var nDecr:int := bs * (p + 1);
+        var span := p * (p + 1);
+        assert sat(i1, countWithinLe(nIncr, incr, span, timefun));
+        assert sat(i1, countWithinGe(nDecr, decr, span, timefun));
+
+        forall i2 {:trigger TLe(i1, i2)} | TLe(i1, i2)
+          ensures || (sat(i2, PacketDeliveredToHostTemporal(b, host)) && !sat(i2, ReceiveAttemptedTemporal(b, host)) && d[i2 + 1] == d[i2] + 1)
+                  || (!sat(i2, PacketDeliveredToHostTemporal(b, host)) && sat(i2, ReceiveAttemptedTemporal(b, host)) && d[i2 + 1] < d[i2])
+                  || (!sat(i2, PacketDeliveredToHostTemporal(b, host)) && !sat(i2, ReceiveAttemptedTemporal(b, host)) && d[i2 + 1] == d[i2]);
+        {
+          Lemma_DeliverIncrReceiveDecr(i1, i2, b, host, d);
+        }
+
+        var i2 := Lemma_CountIncrDecr(i1, d, nIncr, nDecr, incr, decr, span, timefun);
+        assert nDecr > 0;
+        assert TLe(i1, i2 - 1);
+        assert nIncr < nDecr;
+        assert d[i2] < d[i1];
+        assert sat(i2, stepDecrease(i1, d));
+        assert i2 - 1 + 1 == i2;
+        assert sat(i2 - 1 + 1, stepDecrease(i1, d));
+        assert sat(i2 - 1, nextDecrease(i1, d));
+        assert !sat(i2 - 1, nextDecrease(i1, d));
+        assert false; // proof by contradiction
+      }
+      var i2 :| TLe(i1, i2) && sat(i2, or(goal, nextDecrease(i1, d)));
+      assert sat(i1, eventual(or(goal, nextDecrease(i1, d))));
     }
+    assert imaptotal(d);
+    assert forall i :: start <= i ==> 0 <= d[i];
+    assert sat(start, always(nextOrDecrease(goal, d)));
+    Lemma_EventuallyNext(i0, d, goal);
+    assert sat(start, always(eventual(goal)));
+  }
 }
 
-
 lemma Lemma_EventuallyAllPacketsAlwaysReceivedInTimeHelper3<IdType, MessageType>(
-    synchrony_start:int,
-    latency_bound:int,
-    sources:set<IdType>,
-    destinations:set<IdType>,
-    b:Behavior<LEnvironment<IdType, MessageType>>,
-    burst_size:int,
-    receive_period:int
-    ) returns
-    (processing_bound:int)
-    requires imaptotal(b);
-    requires LEnvironment_BehaviorSatisfiesSpec(b);
-    requires HostQueuesLive(b);
-    requires TLe(0, synchrony_start);
-    requires 1 <= receive_period;
-    requires 1 <= burst_size;
+  synchrony_start:int,
+  latency_bound:int,
+  sources:set<IdType>,
+  destinations:set<IdType>,
+  b:Behavior<LEnvironment<IdType, MessageType>>,
+  burst_size:int,
+  receive_period:int
+  ) returns
+  (processing_bound:int)
+  requires imaptotal(b)
+  requires LEnvironment_BehaviorSatisfiesSpec(b)
+  requires HostQueuesLive(b)
+  requires TLe(0, synchrony_start)
+  requires 1 <= receive_period
+  requires 1 <= burst_size
 
-    // Eventually we reach a point where packets sent between these hosts are delivered within latency_bound.
-    requires sat(synchrony_start, always(PacketsSynchronousForHostsTemporal(b, latency_bound, sources, destinations)));
+  // Eventually we reach a point where packets sent between these hosts are delivered within latency_bound.
+  requires sat(synchrony_start, always(PacketsSynchronousForHostsTemporal(b, latency_bound, sources, destinations)))
 
-    // Each of the destinations eventually reaches a point where it attempts to receive a packet at least once every receive_period.
-    // That is, it performs an I/O that's either a Receive or a TimeoutReceive.
-    requires forall host :: host in destinations ==> sat(synchrony_start, always(eventuallynextwithin(ReceiveAttemptedTemporal(b, host), receive_period, BehaviorToTimeMap(b))));
+  // Each of the destinations eventually reaches a point where it attempts to receive a packet at least once every receive_period.
+  // That is, it performs an I/O that's either a Receive or a TimeoutReceive.
+  requires forall host :: host in destinations ==> sat(synchrony_start, always(eventuallynextwithin(ReceiveAttemptedTemporal(b, host), receive_period, BehaviorToTimeMap(b))))
 
-    requires forall host :: host in destinations ==> sat(synchrony_start, always(QueueBounded(b, host, burst_size)));
+  requires forall host :: host in destinations ==> sat(synchrony_start, always(QueueBounded(b, host, burst_size)));
 
-    // Eventually we reach a point where any packet sent between these hosts is received within burst_size *
-    // receive_period after it is sent.
-    ensures  sat(synchrony_start, always(AllPacketsReceivedWithinTemporal(b, latency_bound + burst_size * receive_period, sources, destinations)));
-    ensures  processing_bound == latency_bound + burst_size * receive_period;
+  // Eventually we reach a point where any packet sent between these hosts is received within burst_size *
+  // receive_period after it is sent.
+  ensures  sat(synchrony_start, always(AllPacketsReceivedWithinTemporal(b, latency_bound + burst_size * receive_period, sources, destinations)))
+  ensures  processing_bound == latency_bound + burst_size * receive_period
 {
-    forall i1 | TLe(synchrony_start, i1)
-        ensures sat(i1, AllPacketsReceivedWithinTemporal(b, latency_bound + burst_size * receive_period, sources, destinations));
+  forall i1 | TLe(synchrony_start, i1)
+    ensures sat(i1, AllPacketsReceivedWithinTemporal(b, latency_bound + burst_size * receive_period, sources, destinations))
+  {
+    forall p {:trigger PacketSentBetweenHosts(b[i1], p, sources, destinations)} | PacketSentBetweenHosts(b[i1], p, sources, destinations)
+      ensures sat(i1, next(eventuallynextwithin(PacketReceivedTemporal(b, p), latency_bound + burst_size * receive_period, BehaviorToTimeMap(b))))
     {
-        forall p {:trigger PacketSentBetweenHosts(b[i1], p, sources, destinations)} | PacketSentBetweenHosts(b[i1], p, sources, destinations)
-            ensures sat(i1, next(eventuallynextwithin(PacketReceivedTemporal(b, p), latency_bound + burst_size * receive_period, BehaviorToTimeMap(b))));
-        {
-            var timefun := BehaviorToTimeMap(b);
-            var bs := burst_size;
-            var r := receive_period;
-            var lb := latency_bound;
-            var goal := PacketReceivedTemporal(b, p);
-            assert p.dst in destinations;
+      var timefun := BehaviorToTimeMap(b);
+      var bs := burst_size;
+      var r := receive_period;
+      var lb := latency_bound;
+      var goal := PacketReceivedTemporal(b, p);
+      assert p.dst in destinations;
 
-            forall ensures exists i2 :: TLe(i1, i2) && sat(i2, PacketDeliveredTemporal(b, p)) && timefun[i2 + 1] <= timefun[i1+1] + lb;
-            {
-                TemporalAssist();
-                assert sat(i1+1, eventuallynextwithin(PacketDeliveredTemporal(b, p), latency_bound, BehaviorToTimeMap(b)));
-            }
-            var i2 :| TLe(i1, i2) && sat(i2, PacketDeliveredTemporal(b, p)) && timefun[i2 + 1] <= timefun[i1+1] + lb;
-            TemporalDeduceFromAlways(0, i2, HostQueuesNextTemporal(b));
-            var d := imap i ::
+      forall ensures (exists i2 :: TLe(i1, i2) && sat(i2, PacketDeliveredTemporal(b, p)) && timefun[i2 + 1] <= timefun[i1+1] + lb)
+      {
+        TemporalDeduceFromAlways(synchrony_start, i1, PacketsSynchronousForHostsTemporal(b, latency_bound, sources, destinations));
+        TemporalDeduceFromAlways(0, i1, EnvironmentNextTemporal(b));
+        assert p in b[i1 + 1].sentPackets;
+        var i2 := TemporalDeduceFromEventual(i1 + 1, nextbefore(PacketDeliveredTemporal(b, p), timefun[i1 + 1] + lb, timefun));
+        Lemma_TimeOnlyAdvancesBetweenSteps(b, i2, i2 + 1);
+      }
+      var i2 :| TLe(i1, i2) && sat(i2, PacketDeliveredTemporal(b, p)) && timefun[i2 + 1] <= timefun[i1+1] + lb;
+      TemporalDeduceFromAlways(0, i2, HostQueuesNextTemporal(b));
+      var d := imap i ::
                 (if TLe(i2, i) && p.dst in b[i].hostInfo && p in b[i].hostInfo[p.dst].queue
                     then 1 + QueuePosition(b[i].hostInfo[p.dst].queue, p)
                     else 0);
-            forall ensures sat(i2 + 1, eventuallynextwithin(goal, r * bs, timefun));
-            {
-                assert p in b[i2 + 1].hostInfo[p.dst].queue;
-                assert TLe(synchrony_start, i2 + 1);
-                forall i | TLe(synchrony_start, i) && p.dst in b[i].hostInfo
-                    ensures |b[i].hostInfo[p.dst].queue| <= bs;
-                {
-                    TemporalAssist();
-                    assert TLe(synchrony_start, i);
-                    TemporalDeduceFromAlways(synchrony_start, i, QueueBounded(b, p.dst, bs));
-                    assert |b[i].hostInfo[p.dst].queue| <= bs;
-                }
-                forall i3 | TLe(i2 + 1, i3)
-                    ensures sat(i3, actionGoalDecreaseWithin(goal, d, r, timefun));
-                {
-                    TemporalAssist();
-                    assert TLe(synchrony_start, i3);
-                    assert sat(i3, eventuallynextwithin(ReceiveAttemptedTemporal(b, p.dst), r, timefun));
-                    Lemma_EstablishMonotonicFromOpaque(b, i3);
-                    reveal_monotonic_from_opaque();
-                    var i4 := Lemma_ReceiveAttemptDecr(i2, i3, b, p, d, r, timefun);
-                    assert sat(i3, actionGoalDecreaseWithin(goal, d, r, timefun));
-                }
-                forall ensures sat(i2 + 1, eventuallynextwithinspans(d, goal, r, timefun));
-                {
-                    forall ensures sat(i2 + 1, always(actionGoalDecreaseWithin(goal, d, r, timefun)));
-                    {
-                        TemporalAssist();
-                        assert forall i3 :: TLe(i2 + 1, i3) ==> sat(i3, actionGoalDecreaseWithin(goal, d, r, timefun));
-                        assert sat(i2 + 1, always(actionGoalDecreaseWithin(goal, d, r, timefun)));
-                    }
-                    Lemma_EventuallyNextGoalSpans(i2 + 1, d, goal, r, timefun);
-                }
-                forall ensures sat(i2 + 1, eventuallynextwithin(goal, r * bs, timefun));
-                {
-                    TemporalAssist();
-                    assert sat(i2 + 1, eventuallynextwithinspans(d, goal, r, timefun));
-                    assert sat(i2 + 1, eventuallynextwithin(goal, r * d[i2 + 1], timefun));
-                    assert d[i2 + 1] <= bs;
-                    forall ensures r * d[i2 + 1] <= r * bs { lemma_mul_inequality_forall(); lemma_mul_auto(); }
-                    assert sat(i2 + 1, eventuallynextwithin(goal, r * bs, timefun));
-                }
-            }
-            forall ensures sat(i1, next(eventuallynextwithin(goal, lb + bs * r, timefun)))
-            {
-                TemporalAssist();
-                var i3 :| TLe(i2 + 1, i3) && sat(i3, goal) && timefun[i3 + 1] <= timefun[i2 + 1] + r * bs;
-                assert TLe(i1, i3);
-                forall ensures bs * r == r * bs { lemma_mul_auto(); }
-            }
+      forall ensures sat(i2 + 1, eventuallynextwithin(goal, r * bs, timefun))
+      {
+        assert p in b[i2 + 1].hostInfo[p.dst].queue;
+        assert TLe(synchrony_start, i2 + 1);
+        forall i | TLe(synchrony_start, i) && p.dst in b[i].hostInfo
+          ensures |b[i].hostInfo[p.dst].queue| <= bs
+        {
+          TemporalAssist();
+          assert TLe(synchrony_start, i);
+          TemporalDeduceFromAlways(synchrony_start, i, QueueBounded(b, p.dst, bs));
+          assert |b[i].hostInfo[p.dst].queue| <= bs;
         }
-    }
-    forall ensures sat(synchrony_start, always(AllPacketsReceivedWithinTemporal(b, latency_bound + burst_size * receive_period, sources, destinations)));
-    {
+        forall i3 | TLe(i2 + 1, i3)
+          ensures sat(i3, actionGoalDecreaseWithin(goal, d, r, timefun))
+        {
+          TemporalAssist();
+          assert TLe(synchrony_start, i3);
+          assert sat(i3, eventuallynextwithin(ReceiveAttemptedTemporal(b, p.dst), r, timefun));
+          Lemma_EstablishMonotonicFromOpaque(b, i3);
+          reveal monotonic_from_opaque();
+          var i4 := Lemma_ReceiveAttemptDecr(i2, i3, b, p, d, r, timefun);
+          assert sat(i3, actionGoalDecreaseWithin(goal, d, r, timefun));
+        }
+        forall ensures sat(i2 + 1, eventuallynextwithinspans(d, goal, r, timefun))
+        {
+          forall ensures sat(i2 + 1, always(actionGoalDecreaseWithin(goal, d, r, timefun)))
+          {
+            TemporalAssist();
+            assert forall i3 :: TLe(i2 + 1, i3) ==> sat(i3, actionGoalDecreaseWithin(goal, d, r, timefun));
+            assert sat(i2 + 1, always(actionGoalDecreaseWithin(goal, d, r, timefun)));
+          }
+          Lemma_EventuallyNextGoalSpans(i2 + 1, d, goal, r, timefun);
+        }
+        forall ensures sat(i2 + 1, eventuallynextwithin(goal, r * bs, timefun))
+        {
+          TemporalAssist();
+          assert sat(i2 + 1, eventuallynextwithinspans(d, goal, r, timefun));
+          assert sat(i2 + 1, eventuallynextwithin(goal, r * d[i2 + 1], timefun));
+          assert d[i2 + 1] <= bs;
+          forall ensures r * d[i2 + 1] <= r * bs { lemma_mul_inequality_forall(); lemma_mul_auto(); }
+          assert sat(i2 + 1, eventuallynextwithin(goal, r * bs, timefun));
+        }
+      }
+      forall ensures sat(i1, next(eventuallynextwithin(goal, lb + bs * r, timefun)))
+      {
         TemporalAssist();
+        var i3 :| TLe(i2 + 1, i3) && sat(i3, goal) && timefun[i3 + 1] <= timefun[i2 + 1] + r * bs;
+        assert TLe(i1, i3);
+        forall ensures bs * r == r * bs { lemma_mul_auto(); }
+      }
     }
+  }
+  forall ensures sat(synchrony_start, always(AllPacketsReceivedWithinTemporal(b, latency_bound + burst_size * receive_period, sources, destinations)))
+  {
+    TemporalAssist();
+  }
 
-    processing_bound := latency_bound + burst_size * receive_period;
+  processing_bound := latency_bound + burst_size * receive_period;
 }
 
 lemma Lemma_EventuallyAllPacketsAlwaysReceivedInTimeHelper2<IdType, MessageType>(
-    synchrony_start:int,
-    i1:int,
-    latency_bound:int,
-    sources:set<IdType>,
-    destinations:set<IdType>,
-    b:Behavior<LEnvironment<IdType, MessageType>>,
-    burst_size:int,
-    receive_period:int
-    ) returns
-    (processing_sync_start:int,
-     processing_bound:int)
-    requires imaptotal(b);
-    requires LEnvironment_BehaviorSatisfiesSpec(b);
-    requires HostQueuesLive(b);
-    requires TLe(0, synchrony_start);
-    requires TLe(synchrony_start, i1);
-    requires 1 <= receive_period;
-    requires 1 <= burst_size;
+  synchrony_start:int,
+  i1:int,
+  latency_bound:int,
+  sources:set<IdType>,
+  destinations:set<IdType>,
+  b:Behavior<LEnvironment<IdType, MessageType>>,
+  burst_size:int,
+  receive_period:int
+  ) returns (
+  processing_sync_start:int,
+  processing_bound:int
+  )
+  requires imaptotal(b)
+  requires LEnvironment_BehaviorSatisfiesSpec(b)
+  requires HostQueuesLive(b)
+  requires TLe(0, synchrony_start)
+  requires TLe(synchrony_start, i1)
+  requires 1 <= receive_period
+  requires 1 <= burst_size
 
-    // Eventually we reach a point where packets sent between these hosts are delivered within latency_bound.
-    requires sat(synchrony_start, always(PacketsSynchronousForHostsTemporal(b, latency_bound, sources, destinations)));
+  // Eventually we reach a point where packets sent between these hosts are delivered within latency_bound.
+  requires sat(synchrony_start, always(PacketsSynchronousForHostsTemporal(b, latency_bound, sources, destinations)))
 
-    // Each of the destinations eventually reaches a point where it attempts to receive a packet at least once every receive_period.
-    // That is, it performs an I/O that's either a Receive or a TimeoutReceive.
-    requires forall host :: host in destinations ==> sat(synchrony_start, always(eventuallynextwithin(ReceiveAttemptedTemporal(b, host), receive_period, BehaviorToTimeMap(b))));
+  // Each of the destinations eventually reaches a point where it attempts to receive a packet at least once every receive_period.
+  // That is, it performs an I/O that's either a Receive or a TimeoutReceive.
+  requires forall host :: host in destinations ==> sat(synchrony_start, always(eventuallynextwithin(ReceiveAttemptedTemporal(b, host), receive_period, BehaviorToTimeMap(b))))
 
-    // Each of the destinations eventually reaches a point after which the network stops overwhelming it with
-    // delivered packets.  That is, there are at most burst_size packets delivered to it during any period
-    // of length <= burst_size * receive_period + 1
-    requires forall host :: host in destinations ==> sat(synchrony_start, always(NetworkDeliveryRateForHostBoundedTemporal(b, burst_size, burst_size * receive_period + 1, host)));
+  // Each of the destinations eventually reaches a point after which the network stops overwhelming it with
+  // delivered packets.  That is, there are at most burst_size packets delivered to it during any period
+  // of length <= burst_size * receive_period + 1
+  requires forall host :: host in destinations ==> sat(synchrony_start, always(NetworkDeliveryRateForHostBoundedTemporal(b, burst_size, burst_size * receive_period + 1, host)))
 
-    requires forall host :: host in destinations ==> sat(i1, always(QueueBounded(b, host, burst_size)));
+  requires forall host :: host in destinations ==> sat(i1, always(QueueBounded(b, host, burst_size)))
 
-    // Eventually we reach a point where any packet sent between these hosts is received within burst_size *
-    // receive_period after it is sent.
-    ensures  synchrony_start <= processing_sync_start;
-    ensures  processing_bound == latency_bound + burst_size * receive_period;
-    ensures  sat(processing_sync_start, always(AllPacketsReceivedWithinTemporal(b, latency_bound + burst_size * receive_period, sources, destinations)));
+  // Eventually we reach a point where any packet sent between these hosts is received within burst_size *
+  // receive_period after it is sent.
+  ensures  synchrony_start <= processing_sync_start
+  ensures  processing_bound == latency_bound + burst_size * receive_period
+  ensures  sat(processing_sync_start, always(AllPacketsReceivedWithinTemporal(b, latency_bound + burst_size * receive_period, sources, destinations)))
 {
-    Lemma_AlwaysImpliesLaterAlways(synchrony_start, i1, PacketsSynchronousForHostsTemporal(b, latency_bound, sources, destinations));
-    forall host | host in destinations
-        ensures sat(i1, always(eventuallynextwithin(ReceiveAttemptedTemporal(b, host), receive_period, BehaviorToTimeMap(b))));
-        ensures sat(i1, always(NetworkDeliveryRateForHostBoundedTemporal(b, burst_size, burst_size * receive_period + 1, host)));
-    {
-        Lemma_AlwaysImpliesLaterAlways(synchrony_start, i1, eventuallynextwithin(ReceiveAttemptedTemporal(b, host), receive_period, BehaviorToTimeMap(b)));
-        Lemma_AlwaysImpliesLaterAlways(synchrony_start, i1, NetworkDeliveryRateForHostBoundedTemporal(b, burst_size, burst_size * receive_period + 1, host));
-    }
-    processing_bound := Lemma_EventuallyAllPacketsAlwaysReceivedInTimeHelper3(i1, latency_bound, sources, destinations, b, burst_size, receive_period);
-    processing_sync_start := i1;
+  Lemma_AlwaysImpliesLaterAlways(synchrony_start, i1, PacketsSynchronousForHostsTemporal(b, latency_bound, sources, destinations));
+  forall host | host in destinations
+    ensures sat(i1, always(eventuallynextwithin(ReceiveAttemptedTemporal(b, host), receive_period, BehaviorToTimeMap(b))))
+    ensures sat(i1, always(NetworkDeliveryRateForHostBoundedTemporal(b, burst_size, burst_size * receive_period + 1, host)))
+  {
+    Lemma_AlwaysImpliesLaterAlways(synchrony_start, i1,
+                                   eventuallynextwithin(ReceiveAttemptedTemporal(b, host), receive_period, BehaviorToTimeMap(b)));
+    Lemma_AlwaysImpliesLaterAlways(synchrony_start, i1,
+                                   NetworkDeliveryRateForHostBoundedTemporal(b, burst_size, burst_size * receive_period + 1, host));
+  }
+  processing_bound :=
+    Lemma_EventuallyAllPacketsAlwaysReceivedInTimeHelper3(i1, latency_bound, sources, destinations, b, burst_size, receive_period);
+  processing_sync_start := i1;
 }
 
 lemma Lemma_EventuallyAllPacketsAlwaysReceivedInTime<IdType, MessageType>(
-    synchrony_start:int,
-    latency_bound:int,
-    sources:set<IdType>,
-    destinations:set<IdType>,
-    b:Behavior<LEnvironment<IdType, MessageType>>,
-    burst_size:int,
-    receive_period:int
-    ) returns
-    (processing_sync_start:int,
-     processing_bound:int)
-    requires imaptotal(b);
-    requires LEnvironment_BehaviorSatisfiesSpec(b);
-    requires HostQueuesLive(b);
-    requires TLe(0, synchrony_start);
-    requires 1 <= receive_period;
-    requires 1 <= burst_size;
+  synchrony_start:int,
+  latency_bound:int,
+  sources:set<IdType>,
+  destinations:set<IdType>,
+  b:Behavior<LEnvironment<IdType, MessageType>>,
+  burst_size:int,
+  receive_period:int
+  ) returns (
+  processing_sync_start:int,
+  processing_bound:int
+  )
+  requires imaptotal(b)
+  requires LEnvironment_BehaviorSatisfiesSpec(b)
+  requires HostQueuesLive(b)
+  requires TLe(0, synchrony_start)
+  requires 1 <= receive_period
+  requires 1 <= burst_size
 
-    // All packets sent between these hosts are delivered within latency_bound.
-    requires NetworkSynchronousForHosts(b, synchrony_start, latency_bound, sources, destinations);
+  // All packets sent between these hosts are delivered within latency_bound.
+  requires NetworkSynchronousForHosts(b, synchrony_start, latency_bound, sources, destinations)
 
-    // The network does not overwhelm any of the destinations with delivered packets.  That is,
-    // there are at most burst_size packets delivered to it during any period of
-    // length <= burst_size * receive_period + 1.
-    requires NetworkDeliveryRateBoundedForHosts(b, synchrony_start, burst_size, burst_size * receive_period + 1, destinations);
+  // The network does not overwhelm any of the destinations with delivered packets.  That is,
+  // there are at most burst_size packets delivered to it during any period of
+  // length <= burst_size * receive_period + 1.
+  requires NetworkDeliveryRateBoundedForHosts(b, synchrony_start, burst_size, burst_size * receive_period + 1, destinations)
 
-    // Each of the destinations attempts to receive a packet at least once every receive_period.
-    // That is, it performs an I/O that's either a Receive or a TimeoutReceive.
-    requires forall host :: host in destinations ==> sat(synchrony_start, always(eventuallynextwithin(ReceiveAttemptedTemporal(b, host), receive_period, BehaviorToTimeMap(b))));
+  // Each of the destinations attempts to receive a packet at least once every receive_period.
+  // That is, it performs an I/O that's either a Receive or a TimeoutReceive.
+  requires forall host :: host in destinations ==> sat(synchrony_start, always(eventuallynextwithin(ReceiveAttemptedTemporal(b, host), receive_period, BehaviorToTimeMap(b))))
 
-    // Any packet sent between these hosts is received within burst_size * receive_period after it is sent.
-    ensures  synchrony_start <= processing_sync_start;
-    ensures  processing_bound == latency_bound + burst_size * receive_period;
-    ensures  sat(processing_sync_start, always(AllPacketsReceivedWithinTemporal(b, latency_bound + burst_size * receive_period, sources, destinations)));
+  // Any packet sent between these hosts is received within burst_size * receive_period after it is sent.
+  ensures  synchrony_start <= processing_sync_start
+  ensures  processing_bound == latency_bound + burst_size * receive_period
+  ensures  sat(processing_sync_start, always(AllPacketsReceivedWithinTemporal(b, latency_bound + burst_size * receive_period, sources, destinations)))
 {
-    Lemma_EventuallyEachHostQueueEmpties(latency_bound, destinations, b, synchrony_start, burst_size, receive_period);
+  Lemma_EventuallyEachHostQueueEmpties(latency_bound, destinations, b, synchrony_start, burst_size, receive_period);
 
-    forall host | host in destinations
-        ensures exists i0a :: TLe(synchrony_start, i0a) && sat(i0a, always(QueueBounded(b, host, burst_size)));
-    {
-        TemporalAssist();
-        var i0a :| TLe(synchrony_start, i0a) && sat(i0a, HostQueueEmptyTemporal(b, host));
-        Lemma_HostQueueSizeBoundedAfterEmpty(latency_bound, host, b, i0a, burst_size, receive_period);
-    }
-    var i0as := set host | host in destinations ::
-        (var i0a :| TLe(synchrony_start, i0a) && sat(i0a, always(QueueBounded(b, host, burst_size))); i0a);
-    var i0s := {synchrony_start} + i0as;
-    var i1 := intsetmax(i0s);
+  forall host | host in destinations
+    ensures exists i0a :: TLe(synchrony_start, i0a) && sat(i0a, always(QueueBounded(b, host, burst_size)))
+  {
+    TemporalAssist();
+    var i0a :| TLe(synchrony_start, i0a) && sat(i0a, HostQueueEmptyTemporal(b, host));
+    Lemma_HostQueueSizeBoundedAfterEmpty(latency_bound, host, b, i0a, burst_size, receive_period);
+  }
+  var i0as := set host | host in destinations ::
+                (var i0a :| TLe(synchrony_start, i0a) && sat(i0a, always(QueueBounded(b, host, burst_size))); i0a);
+  var i0s := {synchrony_start} + i0as;
+  var i1 := intsetmax(i0s);
 
-    assert synchrony_start <= i1;
-    assert forall i :: i in i0as ==> i <= i1;
+  assert synchrony_start <= i1;
+  assert forall i :: i in i0as ==> i <= i1;
 
-    forall host | host in destinations
-        ensures sat(i1, always(QueueBounded(b, host, burst_size)));
-    {
-        var i0a :| i0a in i0as && sat(i0a, always(QueueBounded(b, host, burst_size)));
-        assert i0a <= i1;
-        TemporalAssist();
-    }
-    processing_sync_start, processing_bound := Lemma_EventuallyAllPacketsAlwaysReceivedInTimeHelper2(synchrony_start, i1, latency_bound, sources, destinations, b, burst_size, receive_period);
+  forall host | host in destinations
+    ensures sat(i1, always(QueueBounded(b, host, burst_size)))
+  {
+    var i0a :| i0a in i0as && sat(i0a, always(QueueBounded(b, host, burst_size)));
+    assert i0a <= i1;
+    TemporalAssist();
+  }
+  processing_sync_start, processing_bound :=
+    Lemma_EventuallyAllPacketsAlwaysReceivedInTimeHelper2(synchrony_start, i1, latency_bound, sources, destinations,
+                                                          b, burst_size, receive_period);
 }
 
 } 
